Current state of alias analysis

backend/AliasAnalysisDriver.ml
@@ -1,0 +1,55 @@
+open AST
+open BinPos
+open Camlcoq
+open Datatypes
+open Maps
+open Op
+open AliasAnalysis
+open AliasAnalysisPrinters
+open RTL
+
+let cmp_keys x y =
+  match x, y with
+  | (a, _), (b, _) -> compare (int_of_pos b) (int_of_pos a)
+
+(*let printer (k, v) =
+  print_endline (string_of_pos k ^ ": " ^
+                   (string_of_ptmap (coerce_solver v) ^ "\n"))*)
+
+let sorted_map f t =
+  let nodes = PTree.elements t in
+  let sorted_nodes = List.sort cmp_keys nodes in
+  List.map f sorted_nodes
+
+let biprint tnode tres key =
+  match PTree.get key tnode, PTree.get key tres with
+  | None, None   -> assert false
+  | Some n, None -> print_endline ("NO RESULT FOR NODE: " ^ string_of_instr n)
+  | None, Some _ -> assert false
+  | Some node, Some res ->
+      let (rmap, mmap) = coerce_solver res in
+      print_endline (
+        "RMAP: " ^ string_of_rmap rmap ^ "\n"
+               ^ "MMAP: " ^ string_of_mmap mmap ^ "\n"
+               ^ string_of_pos key ^ ": " ^ string_of_instr node
+      )
+
+(* Assuming tnode and tres share the same keys *)
+let sorted_biprint tnode tres =
+  let keys = PTree.xkeys tnode Coq_xH in
+  let sorted_keys =
+    List.sort (fun x y -> compare (int_of_pos y) (int_of_pos x)) keys in
+  List.map (biprint tnode tres) sorted_keys
+
+let alias_analysis fd =
+  match fd with
+  | Internal f ->
+      print_endline ("--------------------");
+      let res = funanalysis f in
+      begin match res with
+      | None            -> print_endline "KILDALL FAILED"
+      | Some (_, ptree) ->
+          let _ = sorted_biprint (fn_code f) ptree in
+          ()
+      end
+  | External _ -> ()
