backend/AliasAnalysisPrinters.ml
@@ -1,0 +1,237 @@
+open AliasAnalysis
+open AST
+open BinInt
+open BinPos
+open Datatypes
+open Maps
+open Op
+open RTL
+
+let rec int_of_pos p =
+  match p with
+  | Coq_xH   -> 1
+  | Coq_xO q -> 2 * int_of_pos q
+  | Coq_xI q -> 2 * int_of_pos q + 1
+
+let string_of_pos p = string_of_int (int_of_pos p)
+
+let string_of_coq_Z z =
+  match z with
+  | Z0 -> "0"
+  | Zpos p -> string_of_pos p
+  | Zneg p -> "-" ^ string_of_pos p
+
+let string_of_node = string_of_pos
+let string_of_ident = string_of_pos
+let string_of_offset = string_of_coq_Z
+let string_of_reg = string_of_pos
+
+let string_of_absb' b =
+  match b with
+  | Allocs(Some n)  -> "Alloc" ^ string_of_node n
+  | Allocs(None)    -> "Allocs"
+  | Globals(Some i) -> "Global" ^ string_of_ident i
+  | Globals(None)   -> "Globals"
+  | Other           -> "Other"
+  | Stack           -> "Stack"
+
+let string_of_absb b =
+  match b with
+  | None     -> "All"
+  | Some(b') -> string_of_absb' b'
+
+let string_of_absp p =
+  match p with
+  | Blk(b)    -> "Blk(" ^ string_of_absb b ^ ")"
+  | Loc(b, o) -> "Loc(" ^ string_of_absb b ^ ", " ^ string_of_coq_Z o ^ ")"
+
+let string_of_reg r = "R" ^ string_of_reg r
+
+let string_of_set set_fold string_of_elt s =
+  let folder elt accu =
+    match accu with
+    | "" -> string_of_elt elt
+    | _  -> accu ^ ", " ^ string_of_elt elt
+  in "{" ^ set_fold folder s "" ^ "}"
+
+let string_of_ptset s =
+  if PTSet.beq s PTSet.top
+  then "⊤"
+  else if PTSet.beq s PTSet.bot
+  then "⊥"
+  else string_of_set PTSet.AbsPSet.fold string_of_absp s
+
+let string_of_rmap (rmap: RMap.t) =
+  match rmap with
+  | None -> "⊤"
+  | Some rmap' ->
+      "{"
+      ^ RMapWithoutTop.M.fold
+        (fun k v accu ->
+          if PTSet.beq v PTSet.bot
+          then accu
+          else
+            (if accu = "" then "" else accu ^ ", ")
+            ^ string_of_reg k ^ " -> " ^ string_of_ptset v
+        )
+        rmap'
+        ""
+      ^ "}"
+
+let string_of_mmap (mmap: MMap.t) =
+  match mmap with
+  | None -> "⊤"
+  | Some mmap' ->
+      "{"
+      ^ MMap.MSL.M.fold
+        (fun k v accu ->
+          (if accu = "" then "" else accu ^ ", ")
+          ^ string_of_absp k ^ " -> " ^ string_of_ptset v
+        )
+        mmap'
+        ""
+      ^ "}"
+
+let string_of_list string_of_elt l =
+  let rec string_of_list_aux l =
+    match l with
+    | []      -> ""
+    | h::rest -> ", " ^ string_of_elt h ^ string_of_list_aux rest
+  in match l with
+  | []      -> "[]"
+  | h::rest -> "[" ^ string_of_elt h ^ string_of_list_aux rest ^ "]"
+
+let string_of_reglist = string_of_list string_of_reg
+
+let string_of_sum string_of_left string_of_right s =
+  match s with
+  | Coq_inl l -> string_of_left l
+  | Coq_inr r -> string_of_right r
+
+let string_of_reg_ident_sum = string_of_sum string_of_reg string_of_ident
+
+let string_of_option string_of_elt o =
+  match o with
+  | None   -> "None"
+  | Some e -> "Some " ^ string_of_elt e
+
+let string_of_reg_option = string_of_option string_of_reg
+
+let string_of_addr a =
+  match a with
+  | Aindexed o             -> "Aindexed " ^ string_of_coq_Z o
+  | Aindexed2 o            -> "Aindexed2 " ^ string_of_coq_Z o
+  | Ascaled (s, o)         ->
+      "Ascaled (" ^ string_of_coq_Z s ^ ", " ^ string_of_coq_Z o ^ ")"
+  | Aindexed2scaled (s, o) ->
+      "Aindexed2scaled (" ^ string_of_coq_Z s ^ ", " ^ string_of_coq_Z o ^
+      ")"
+  | Aglobal (i, o)         ->
+      "Aglobal (" ^ string_of_ident i ^ ", " ^ string_of_coq_Z o ^ ")"
+  | Abased (i, o)          ->
+      "Abased (" ^ string_of_ident i ^ ", " ^ string_of_coq_Z o ^ ")"
+  | Abasedscaled (o, i, s) ->
+      "Abasedscaled (" ^ string_of_coq_Z o ^ ", " ^ string_of_ident i ^
+      ", " ^ string_of_coq_Z s ^ ")"
+  | Ainstack o             -> "Ainstack " ^ string_of_coq_Z o
+
+let string_of_op o =
+  match o with
+  | Omove           -> "Omove"
+  | Ointconst i     -> "Ointconst " ^ string_of_coq_Z i
+  | Ofloatconst f   -> "Ofloatconst "
+  | Ocast8signed    -> "Ocast8signed"
+  | Ocast8unsigned  -> "Ocast8unsigned"
+  | Ocast16signed   -> "Ocast16signed"
+  | Ocast16unsigned -> "Ocast16unsigned"
+  | Oneg            -> "Oneg"
+  | Osub            -> "Osub"
+  | Omul            -> "Omul"
+  | Omulimm i       -> "Omulimm " ^ string_of_coq_Z i
+  | Odiv            -> "Odiv"
+  | Odivu           -> "Odivu"
+  | Omod            -> "Omod"
+  | Omodu           -> "Omodu"
+  | Oand            -> "Oand"
+  | Oandimm i       -> "Oandimm " ^ string_of_coq_Z i
+  | Oor             -> "Oor"
+  | Oorimm i        -> "Oorimm " ^ string_of_coq_Z i
+  | Oxor            -> "Oxor"
+  | Oxorimm i       -> "Oxorimm " ^ string_of_coq_Z i
+  | Oshl            -> "Oshl"
+  | Oshlimm i       -> "Oshlimm " ^ string_of_coq_Z i
+  | Oshr            -> "Oshr"
+  | Oshrimm i       -> "Oshrimm " ^ string_of_coq_Z i
+  | Oshrximm i      -> "Oshrximm " ^ string_of_coq_Z i
+  | Oshru           -> "Oshru"
+  | Oshruimm i      -> "Oshruimm " ^ string_of_coq_Z i
+  | Ororimm i       -> "Ororimm " ^ string_of_coq_Z i
+  | Olea a          -> "Olea " ^ string_of_addr a
+  | Onegf           -> "Onegf"
+  | Oabsf           -> "Oabsf"
+  | Oaddf           -> "Oaddf"
+  | Osubf           -> "Osubf"
+  | Omulf           -> "Omulf"
+  | Odivf           -> "Odivf"
+  | Osingleoffloat  -> "Osingleoffloat"
+  | Ointoffloat     -> "Ointoffloat"
+  | Ofloatofint     -> "Ofloatofint"
+  | Ocmp c          -> "Ocmp "
+
+let string_of_chunk c =
+  match c with
+  | Mint8signed    -> "Mint8signed"
+  | Mint8unsigned  -> "Mint8unsigned"
+  | Mint16signed   -> "Mint16signed"
+  | Mint16unsigned -> "Mint16unsigned"
+  | Mint32         -> "Mint32"
+  | Mfloat32       -> "Mfloat32"
+  | Mfloat64       -> "Mfloat64"
+
+let string_of_external ef =
+  match ef with
+  | EF_external (i, _)        -> "External " ^ string_of_ident i
+  | EF_builtin (i, _)         -> "Builtin " ^ string_of_ident i
+  | EF_vload _                -> "VLoad"
+  | EF_vstore _               -> "VStore"
+  | EF_vload_global(_, i, _)  -> "VLoadGlobal " ^ string_of_ident i
+  | EF_vstore_global(_, i, _) -> "VStoreGlobal " ^ string_of_ident i
+  | EF_malloc                 -> "Malloc"
+  | EF_free                   -> "Free"
+  | EF_memcpy (_, _)          -> "Memcpy"
+  | EF_annot (_, _)           -> "Annotation"
+  | EF_annot_val (_, _)       -> "Annotation"
+
+let string_of_instr i =
+  match i with
+  | Inop succ                             ->
+      "Inop {succ: " ^ string_of_node succ ^ "}"
+  | Iop (op, args, dest, succ)            ->
+      "Iop {op: " ^ string_of_op op ^ "} {args: " ^ string_of_reglist args ^
+      "} {dest: " ^ string_of_reg dest ^ "} {succ: " ^ string_of_node succ ^ "}"
+  | Iload (chunk, addr, args, dest, succ) ->
+      "Iload {chunk: " ^ string_of_chunk chunk ^ "} {addr: " ^
+      string_of_addr addr ^ "} {args: " ^ string_of_reglist args ^
+      "} {dest:" ^ string_of_reg dest ^ "} {succ: " ^ string_of_node succ ^ "}"
+  | Istore (chunk, addr, args, src, succ) ->
+      "Istore {chunk: " ^ string_of_chunk chunk ^ "} {addr: " ^
+      string_of_addr addr ^ "} {args: " ^ string_of_reglist args ^ "} {src: " ^
+      string_of_reg src ^ "} {succ: " ^ string_of_node succ ^ "}"
+  | Icall (sign, fn, args, dest, succ)    ->
+      "Icall {fn: " ^ string_of_reg_ident_sum fn ^ "} {args: " ^
+      string_of_reglist args ^ "} {dest: " ^ string_of_reg dest ^ "} {succ: " ^
+      string_of_node succ ^ "}"
+  | Itailcall (sign, fn, args)            ->
+      "Itailcall {fn: " ^ string_of_reg_ident_sum fn ^ "} {args: " ^
+      string_of_reglist args ^ "}"
+  | Ibuiltin (ef, args, dest, succ)       ->
+      "Ibuiltin {ef: " ^ string_of_external ef ^ "} {args: " ^
+      string_of_reglist args ^ "} {dest: " ^ string_of_reg dest ^ "} {succ: " ^
+      string_of_node succ ^ "}"
+  | Icond (cond, args, ifso, ifnot)       ->
+      "Icond {args: " ^ string_of_reglist args ^ "} {ifso: " ^
+      string_of_node ifso ^ "} {ifnot: " ^ string_of_node ifnot ^ "}"
+  | Ijumptable (arg, tbl)                 ->
+      "Ijumptable {}"
+  | Ireturn r                             ->
+      "Ireturn {r: " ^ string_of_reg_option r ^ "}"
