backend/AliasAnalysis.v
@@ -1,0 +1,2813 @@
+Require Import AST.
+Require Import Coqlib.
+Require Import FMapAVL.
+Require FMapFacts.
+Require Import FMapInterface.
+Require FSetFacts.
+Require Import Globalenvs.
+Require Import Integers.
+Require Import Lattice.
+Require Import List.
+Require Import Maps.
+Require Import Memory.
+Require Import Op.
+Require Import Kildall.
+Require Import Registers.
+Require Import RTL.
+Require Import Values.
+
+(* Library *)
+
+Require String. Open Scope string_scope.
+Ltac move_to_top x :=
+  match reverse goal with
+  | H : _ |- _ => try move x after H
+  end.
+Tactic Notation "assert_eq" ident(x) constr(v) :=
+  let H := fresh in
+  assert (x = v) as H by reflexivity;
+  clear H.
+Tactic Notation "Case_aux" ident(x) constr(name) :=
+  first [
+    set (x := name); move_to_top x
+  | assert_eq x name; move_to_top x
+  | fail 1 "because we are working on a different case" ].
+Tactic Notation "Case" constr(name) := Case_aux Case name.
+Tactic Notation "SCase" constr(name) := Case_aux SCase name.
+Tactic Notation "SSCase" constr(name) := Case_aux SSCase name.
+Tactic Notation "SSSCase" constr(name) := Case_aux SSSCase name.
+Tactic Notation "SSSSCase" constr(name) := Case_aux SSSSCase name.
+Tactic Notation "SSSSSCase" constr(name) := Case_aux SSSSSCase name.
+Tactic Notation "SSSSSSCase" constr(name) := Case_aux SSSSSSCase name.
+Tactic Notation "SSSSSSSCase" constr(name) := Case_aux SSSSSSSCase name.
+Tactic Notation "SSSSSSSSCase" constr(name) := Case_aux SSSSSSSSCase name.
+Tactic Notation "SSSSSSSSSCase" constr(name) := Case_aux SSSSSSSSSCase name.
+
+Ltac unalias := repeat (autounfold with unalias in *).
+
+Ltac feed H :=
+  match type of H with
+  | ?foo -> _ =>
+    let FOO := fresh in
+    assert foo as FOO; [|specialize (H FOO); clear FOO]
+  end.
+
+Ltac feed_all H := feed H; [|try feed_all H].
+
+Ltac feed_n n H :=
+  match constr:n with
+  | O => idtac
+  | (S ?m) => feed H ; [| feed_n m H]
+  end.
+
+(* Interfaces *)
+
+Module Type Hierarchy.
+  Parameter t: Type.
+  Parameter top: t.
+  Parameter parent: t -> option t.
+  Parameter measure: t -> nat.
+  Axiom eq_dec: forall (x y: t), {eq x y} + {~eq x y}. (* useful for optint *)
+  Axiom hierarchy: t -> t -> Prop.
+  Axiom hierarchy_dec: forall x y, {hierarchy x y} + {~ hierarchy x y}.
+  Axiom top_spec: forall x, x <> top -> hierarchy top x.
+  Axiom parent_measure: forall x px,
+    parent x = Some px -> measure x = S (measure px).
+End Hierarchy.
+
+Module Type Overlap.
+  Include Hierarchy.
+  Axiom overlap: t -> t -> Prop.
+  Axiom overlap_dec: forall x y, {overlap x y} + {~ overlap x y}.
+End Overlap.
+
+(* A hierarchical set is a set over hierarchical elements, such that an element
+   up in the hierarchy embodies all of its ancestors. *)
+
+Module Type HSet (H: Hierarchy).
+  Parameter t: Type.
+  Parameter bot: t.
+  Parameter top: t.
+  Parameter add: H.t -> t -> t.
+  Parameter In: H.t -> t -> Prop.
+  Parameter mem: forall x s, {In x s} + {~In x s}.
+  Definition eq (s1 s2: t): Prop := forall x, In x s1 <-> In x s2.
+  Axiom In_add_same: forall x s, In x (add x s).
+  Axiom In_add_hierarchy: forall x y,
+    H.hierarchy x y -> (forall s, In y (add x s)).
+  Axiom In_add_already: forall x y s, In x s -> In x (add y s).
+  Definition singleton x := add x bot.
+  Axiom In_singleton: forall x, In x (singleton x).
+  Axiom In_singleton_hierarchy: forall x y,
+    H.hierarchy x y -> In y (singleton x).
+End HSet.
+
+Module Type OMap (O: Overlap) (L: SEMILATTICE).
+  Parameter t: Type.
+  Parameter get: O.t -> t -> L.t.
+  Parameter add: O.t -> L.t -> t -> t.
+  (* set should only work for keys at the bottom of the hierarchy *)
+  (* set still needs to propagate information upwards *)
+  (*
+    Parameter set: O.t -> L.t -> t -> t.
+  *)
+  Axiom get_add_same: forall k s m, L.ge (get k (add k s m)) s.
+  Axiom get_add: forall x y s m, L.ge (get x (add y s m)) (get x m).
+  Axiom get_add_overlap: forall x y s m,
+    O.overlap x y ->
+    L.ge (get x (add y s m)) s.
+  (*
+  Axiom get_set_same: forall k s m, L.ge (get k (set k s m)) s.
+  Axiom get_set_other: forall x y s m, L.ge (get x (set y s m)) (get x m).
+  *)
+End OMap.
+
+(* Useful functors *)
+
+Module HtoO (H: Hierarchy) <: Overlap.
+  Include H.
+  Definition overlap x y := hierarchy x y \/ hierarchy y x.
+  Definition overlap_dec: forall x y, {overlap x y} + {~ overlap x y}.
+  Proof.
+    intros. destruct (hierarchy_dec x y).
+    left. left. auto. destruct (hierarchy_dec y x).
+    left. right. auto.
+    right. intro. inv H; contradiction.
+  Defined.
+End HtoO.
+
+Module ProductSemiLattice (A: SEMILATTICE) (B: SEMILATTICE) <: SEMILATTICE.
+  Definition t := (A.t * B.t)%type.
+  Definition eq (x y: t) :=
+    let (a, b) := x in let (c, d) := y in
+    A.eq a c /\ B.eq b d.
+  Theorem eq_refl: forall x, eq x x.
+  Proof.
+    destruct x. split. apply A.eq_refl. apply B.eq_refl.
+  Qed.
+  Theorem eq_sym: forall x y, eq x y -> eq y x.
+  Proof.
+    intros. destruct x, y. inv H. constructor.
+    apply A.eq_sym. auto.
+    apply B.eq_sym. auto.
+  Qed.
+  Theorem eq_trans: forall x y z, eq x y -> eq y z -> eq x z.
+  Proof.
+    intros. destruct x, y, z. inv H. inv H0. constructor.
+    eapply A.eq_trans; eauto.
+    eapply B.eq_trans; eauto.
+  Qed.
+  Definition beq (x y: t) :=
+    let (a, b) := x in let (c, d) := y in
+    (A.beq a c) && (B.beq b d).
+  Theorem beq_correct: forall x y, beq x y = true -> eq x y.
+  Proof.
+    intros. destruct x, y. apply andb_prop in H. destruct H as [? ?]. constructor.
+    apply A.beq_correct. auto.
+    apply B.beq_correct. auto.
+  Qed.
+  Definition ge (x y: t) :=
+    let (a, b) := x in let (c, d) := y in
+    A.ge a c /\ B.ge b d.
+  Theorem ge_refl: forall x y, eq x y -> ge x y.
+  Proof.
+    intros. destruct x, y. inv H. constructor.
+    apply A.ge_refl. auto.
+    apply B.ge_refl. auto.
+  Qed.
+  Theorem ge_trans: forall x y z, ge x y -> ge y z -> ge x z.
+  Proof.
+    intros. destruct x, y, z. inv H. inv H0. constructor.
+    eapply A.ge_trans; eauto.
+    eapply B.ge_trans; eauto.
+  Qed.
+  Definition bot := (A.bot, B.bot).
+  Theorem ge_bot: forall x, ge x bot.
+  Proof.
+    destruct x. constructor. apply A.ge_bot. apply B.ge_bot.
+  Qed.
+  Definition lub (x y: t) :=
+    let (a, b) := x in let (c, d) := y in
+    (A.lub a c, B.lub b d).
+  Theorem ge_lub_left: forall x y, ge (lub x y) x.
+  Proof.
+    destruct x, y. constructor. apply A.ge_lub_left. apply B.ge_lub_left.
+  Qed.
+  Theorem ge_lub_right: forall x y, ge (lub x y) y.
+  Proof.
+    destruct x, y. constructor. apply A.ge_lub_right. apply B.ge_lub_right.
+  Qed.
+End ProductSemiLattice.
+
+Module FMapAVLPlus(X: OrderedType).
+
+Module M := FMapAVL.Make(X).
+
+Include M.
+
+Module FMF := FMapFacts.WFacts_fun X M.
+
+Section MAP2.
+
+Variable elt elt' elt'' : Type.
+Variable f : key -> option elt -> option elt' -> option elt''.
+Hypothesis f_compat: forall x x' o1 o2, X.eq x x' -> f x o1 o2 = f x' o1 o2.
+
+Definition raw_map2i : Raw.t elt -> Raw.t elt' -> Raw.t elt'' :=
+  Raw.map2_opt
+    (fun k d o => f k (Some d) o)
+    (Raw.map_option (fun k d => f k (Some d) None))
+    (Raw.map_option (fun k d' => f k None (Some d'))).
+
+Lemma map2i_bst:
+  forall m1 m2, Raw.bst m1 -> Raw.bst m2 -> Raw.bst (raw_map2i m1 m2).
+Proof.
+  intros. unfold raw_map2i.
+  apply Raw.Proofs.map2_opt_bst with (f0 := f); auto; intros.
+  apply Raw.Proofs.map_option_bst; auto.
+  apply Raw.Proofs.map_option_bst; auto.
+  apply Raw.Proofs.map_option_find; auto.
+  apply Raw.Proofs.map_option_find; auto.
+Qed.
+
+Definition map2i (m1: t elt) (m2: t elt') : t elt'' :=
+  Bst (map2i_bst m1 m2 m1.(is_bst) m2.(is_bst)).
+
+Lemma map2i_1: forall (m: t elt)(m': t elt') (x:key),
+  In x m \/ In x m' ->
+  find x (map2i m m') = f x (find x m) (find x m').
+Proof.
+  unfold find, map2i, In; intros until x. simpl.
+  do 2 rewrite Raw.Proofs.In_alt. unfold raw_map2i. intros.
+  rewrite Raw.Proofs.map2_opt_1 with (f0 := f); auto; intros.
+  apply Raw.Proofs.map_option_bst; auto.
+  apply Raw.Proofs.map_option_bst; auto.
+  apply Raw.Proofs.map_option_find; auto.
+  apply Raw.Proofs.map_option_find; auto.
+  apply is_bst. apply is_bst.
+Qed.
+
+Lemma map2i_2: forall (m: t elt)(m': t elt') (x:key),
+  In x (map2i m m') -> In x m \/ In x m'.
+Proof.
+  unfold In, map2i; intros until x.
+  do 3 rewrite Raw.Proofs.In_alt. simpl. unfold raw_map2i; intros.
+  eapply Raw.Proofs.map2_opt_2 with (f0 := f); eauto; intros.
+  apply Raw.Proofs.map_option_bst; auto.
+  apply Raw.Proofs.map_option_bst; auto.
+  apply Raw.Proofs.map_option_find; auto.
+  apply Raw.Proofs.map_option_find; auto.
+  apply is_bst. apply is_bst.
+Qed.
+
+Lemma map2i_3: forall x m1 m2,
+  (forall k, f k None None = None) ->
+  find x m1 = None ->
+  find x m2 = None ->
+  find x (map2i m1 m2) = None.
+Proof.
+  intros. destruct (find x (map2i m1 m2)) as []_eqn; [|auto].
+  assert (find x (map2i m1 m2) <> None). congruence.
+  apply FMF.in_find_iff in H2. apply map2i_2 in H2. inv H2.
+  apply FMF.in_find_iff in H3. congruence.
+  apply FMF.in_find_iff in H3. congruence.
+Qed.
+
+Lemma map2i_4: forall m m' (H: forall k, f k None None = None) x,
+  find x (map2i m m') = f x (find x m) (find x m').
+Proof.
+  intros. destruct (find x m) as []_eqn.
+  rewrite <- Heqo. apply map2i_1. left. apply FMF.in_find_iff. congruence.
+  destruct (find x m') as []_eqn.
+  rewrite <- Heqo. rewrite <- Heqo0. apply map2i_1.
+  right. apply FMF.in_find_iff. congruence.
+  rewrite H. apply map2i_3; auto.
+Qed.
+
+End MAP2.
+
+End FMapAVLPlus.
+
+Module Type MergeStrategy (KEY: OrderedType) (VAL: SEMILATTICE).
+  Variable f: KEY.t -> option VAL.t -> option VAL.t -> option VAL.t.
+  Axiom f_compat:
+    forall (x x': KEY.t) (o1: option VAL.t) (o2: option VAL.t),
+      KEY.eq x x' -> f x o1 o2 = f x' o1 o2.
+End MergeStrategy.
+
+Module MapSemiLattice
+  (KEY: OrderedType)
+  (VAL: SEMILATTICE)
+  (MGS: MergeStrategy(KEY)(VAL))
+  <: SEMILATTICE.
+  Module M := FMapAVLPlus(KEY).
+  Module FMF := FMapFacts.WFacts_fun KEY M.
+  Definition t := M.t VAL.t.
+  Definition eq (x y: t): Prop :=
+    forall k,
+      match M.find k x, M.find k y with
+      | None, None     => True
+      | Some a, Some b => VAL.eq a b
+      | _, _           => False
+      end.
+  Theorem eq_refl: forall x, eq x x.
+  Proof.
+    repeat intro. destruct M.find. apply VAL.eq_refl. auto.
+  Qed.
+  Theorem eq_sym: forall x y, eq x y -> eq y x.
+  Proof.
+    repeat intro. unalias. specialize (H k).
+    destruct M.find; destruct M.find; auto. apply VAL.eq_sym. auto.
+  Qed.
+  Theorem eq_trans: forall x y z, eq x y -> eq y z -> eq x z.
+  Proof.
+    repeat intro. unalias. specialize (H k). specialize (H0 k).
+    destruct M.find; destruct M.find; destruct M.find; auto.
+    eapply VAL.eq_trans; eauto. contradiction.
+  Qed.
+  Definition beq: t -> t -> bool := M.equal VAL.beq.
+  Theorem beq_correct: forall x y, beq x y = true -> eq x y.
+  Proof.
+    repeat intro. apply M.equal_2 in H. inv H.
+    destruct (M.find k x) as []_eqn; destruct (M.find k y) as []_eqn; auto.
+    apply VAL.beq_correct. eapply H1; apply FMF.find_mapsto_iff; eauto.
+    apply FMF.not_find_in_iff in Heqo0. elim Heqo0. apply H0.
+    apply FMF.in_find_iff. congruence.
+    apply FMF.not_find_in_iff in Heqo. elim Heqo. apply H0.
+    apply FMF.in_find_iff. congruence.
+  Qed.
+  (* Assuming None is the same as B.bot *)
+  Definition ge x y :=
+    forall k,
+      match M.find k x, M.find k y with
+      | None,   None   => True
+      | Some a, Some b => VAL.ge a b
+      | Some _, None   => True
+      | None,   Some b => VAL.ge VAL.bot b
+      end.
+  Theorem ge_refl: forall x y, eq x y -> ge x y.
+  Proof.
+    repeat intro. unalias. specialize (H k).
+    destruct (M.find k x) as []_eqn; destruct (M.find k y) as []_eqn; auto.
+    apply VAL.ge_refl. auto. contradiction.
+  Qed.
+  Theorem ge_trans: forall x y z, ge x y -> ge y z -> ge x z.
+  Proof.
+    repeat intro. unalias. specialize (H k). specialize (H0 k).
+    destruct (M.find k x) as []_eqn; destruct (M.find k y) as []_eqn;
+    destruct (M.find k z) as []_eqn; auto.
+    eapply VAL.ge_trans; eauto.
+    eapply VAL.ge_trans. apply VAL.ge_bot. auto.
+    eapply VAL.ge_trans. eauto. auto.
+  Qed.
+  Definition bot: t := M.empty VAL.t.
+  Theorem ge_bot: forall x, ge x bot.
+  Proof.
+    repeat intro.
+    destruct (M.find k x) as []_eqn; rewrite FMF.empty_o; auto.
+  Qed.
+  Definition lub (m: t) (n: t): t :=
+    M.map2i VAL.t VAL.t VAL.t MGS.f MGS.f_compat m n.
+  Axiom ge_lub_left: forall x y, ge (lub x y) x.
+  Axiom ge_lub_right: forall x y, ge (lub x y) y.
+End MapSemiLattice.
+
+Module SemiLatticeToLattice (S: SEMILATTICE) <: SEMILATTICE_WITH_TOP.
+  Definition t := option S.t.
+  Notation Top := None (only parsing).
+  Definition eq (x y: t) :=
+    match x, y with
+    | Top,    Top    => True
+    | Some a, Some b => S.eq a b
+    | _,      _      => False
+    end.
+  Theorem eq_refl: forall x, eq x x.
+  Proof.
+    destruct x; intuition. apply S.eq_refl.
+  Qed.
+  Theorem eq_sym: forall x y, eq x y -> eq y x.
+  Proof.
+    intros. destruct x, y; simpl in *; intuition. apply S.eq_sym. auto.
+  Qed.
+  Theorem eq_trans: forall x y z, eq x y -> eq y z -> eq x z.
+  Proof.
+    intros. destruct x, y, z; simpl in *; intuition. eapply S.eq_trans; eauto.
+  Qed.
+  Definition beq (x y: t) :=
+    match x, y with
+    | Top,    Top => true
+    | Some a, Some b => S.beq a b
+    | _,      _ => false
+    end.
+  Theorem beq_correct: forall x y, beq x y = true -> eq x y.
+  Proof.
+    intros. destruct x, y; simpl in *; intuition. apply S.beq_correct. auto.
+  Qed.
+  Definition ge (x y: t) :=
+    match x, y with
+    | Top,    _      => True
+    | _,      Top    => False
+    | Some a, Some b => S.ge a b
+    end.
+  Theorem ge_refl: forall x y, eq x y -> ge x y.
+  Proof.
+    intros. destruct x, y; simpl in *; intuition. apply S.ge_refl. auto.
+  Qed.
+  Theorem ge_trans: forall x y z, ge x y -> ge y z -> ge x z.
+  Proof.
+    intros. destruct x, y, z; simpl in *; intuition. eapply S.ge_trans; eauto.
+  Qed.
+  Definition bot := Some S.bot.
+  Theorem ge_bot: forall x, ge x bot.
+  Proof.
+    destruct x; simpl in *; intuition. apply S.ge_bot.
+  Qed.
+  Definition lub (x y: t) :=
+    match x, y with
+    | Top,    _      => Top
+    | _,      Top    => Top
+    | Some a, Some b => Some (S.lub a b)
+    end.
+  Theorem ge_lub_left: forall x y, ge (lub x y) x.
+  Proof.
+    destruct x, y; simpl in *; intuition. apply S.ge_lub_left.
+  Qed.
+  Theorem ge_lub_right: forall x y, ge (lub x y) y.
+  Proof.
+    destruct x, y; simpl in *; intuition. apply S.ge_lub_right.
+  Qed.
+  (* New: *)
+  Definition top := @Top S.t.
+  Theorem ge_top: forall x, ge top x.
+  Proof.
+    destruct x; simpl in *; intuition.
+  Qed.
+End SemiLatticeToLattice.
+
+(* Abstract blocks *)
+
+Inductive absb' :=
+| Allocs:  option node  -> absb'
+| Globals: option ident -> absb'
+| Other
+| Stack
+.
+Definition absb := option absb'. (* None := All *)
+Hint Unfold absb: unalias.
+(* Better use this *)
+Notation All := None (only parsing).
+Notation Just := Some (only parsing).
+
+Module AbsBOT <: OrderedType.
+  Definition t := absb.
+  Definition eq := @eq t.
+  Definition eq_refl := @refl_equal t.
+  Definition eq_sym := @sym_eq t.
+  Definition eq_trans := @trans_eq t.
+  Definition eq_dec : forall x y, {eq x y}+{~eq x y}.
+  Proof.
+    unfold eq. destruct x, y; repeat decide equality. left. auto.
+  Defined.
+  Definition lt (x y: t) : Prop :=
+    match x, y with
+    | All,    All    => False
+    | _,      All    => True
+    | All,    _      => False
+    | Just a, Just b =>
+      match a, b with
+      | Allocs (Just n1),  Allocs (Just n2)                         => (n1 < n2)%positive
+      | Allocs (Just _),   (Allocs All | Globals _ | Other | Stack) => True
+      | Allocs All,        (Globals _ | Other | Stack)              => True
+      | Globals (Just g1), Globals (Just g2)                        => (g1 < g2)%positive
+      | Globals (Just _),  (Globals _ | Other | Stack)              => True
+      | Globals All,       (Other | Stack)                          => True
+      | Other,             Stack                                    => True
+      | _,                 _                                        => False
+      end
+    end.
+  Theorem lt_trans : forall x y z, lt x y -> lt y z -> lt x z.
+  Proof.
+    intros.
+    destruct x, y, z;
+    try destruct a; try destruct a0; try destruct a1;
+    try destruct o; try destruct o0; try destruct o1;
+    auto; simpl in *; zify; omega.
+  Qed.
+  Theorem lt_not_eq : forall x y : t, lt x y -> ~ eq x y.
+  Proof.
+    repeat intro. inv H0. destruct y; simpl in H; auto.
+    destruct a; auto; destruct o; auto;  zify; omega.
+  Qed.
+  Definition compare : forall x y : t, Compare lt eq x y.
+  Proof.
+    intros. unfold lt.
+    destruct x, y;
+    try destruct a, a0;
+    try destruct o; try destruct o0;
+    try solve [apply LT; auto|apply EQ; reflexivity|apply GT; auto].
+    destruct (Pcompare n n0 Eq) as []_eqn.
+    apply Pcompare_eq_iff in Heqc; subst; apply EQ; reflexivity.
+    apply LT. auto.
+    pose proof (Pcompare_antisym n n0 Eq). unfold CompOpp in *.
+    apply GT; rewrite Heqc in H.
+    unfold BinPos.Plt. auto.
+    destruct (Pcompare i i0 Eq) as []_eqn.
+    apply Pcompare_eq_iff in Heqc; subst; apply EQ; reflexivity.
+    apply LT; auto.
+    pose proof (Pcompare_antisym i i0 Eq). unfold CompOpp in *.
+    apply GT; rewrite Heqc in H.
+    unfold BinPos.Plt. auto.
+  Defined.
+End AbsBOT.
+
+Module AbsBH <: Hierarchy.
+  Definition t := absb.
+  Definition top: t := None.
+  Definition hierarchy x y :=
+    match x, y with
+    | _,      All    => False
+    | All,    _      => True
+    | Just a, Just b =>
+      match a, b with
+      | Allocs All,  Allocs (Just _)  => True
+      | Globals All, Globals (Just _) => True
+      | _,           _                => False
+      end
+    end.
+  Definition parent x :=
+    match x with
+    | All    => None
+    | Just a => Some (
+      match a with
+      | Allocs (Just _)  => Just (Allocs All)
+      | Globals (Just _) => Just (Globals All)
+      | _                => All
+      end
+    )
+    end.
+  Definition measure x :=
+    (
+    match x with
+    | All    => 0
+    | Just a =>
+      match a with
+      | Allocs (Just _)  => 2
+      | Globals (Just _) => 2
+      | _                => 1
+      end
+    end
+    )%nat.
+  Definition eq_dec: forall (x y: t), {eq x y} + {~ eq x y}.
+  Proof.
+    repeat decide equality.
+  Defined.
+  Definition hierarchy_dec: forall x y, {hierarchy x y} + {~ hierarchy x y}.
+  Proof.
+    intros.
+    destruct x, y; try destruct a, a0; try destruct o; try destruct o0;
+      simpl; auto.
+  Defined.
+  Theorem top_spec: forall x, x <> top -> hierarchy top x.
+  Proof.
+    destruct x; simpl; intuition.
+  Qed.
+  Theorem parent_measure: forall x px,
+    parent x = Some px -> measure x = S (measure px).
+  Proof.
+    intros. destruct x; try destruct a; try destruct o; inv H; auto.
+  Qed.
+End AbsBH.
+
+(* With offsets *)
+
+Inductive optint {t: Type}: Type :=
+| Blk: t -> optint
+| Loc: t -> Int.int -> optint
+.
+Definition absp := @optint absb.
+
+Module OptIntH (H: Hierarchy) <: Hierarchy.
+  Definition t:= @optint H.t.
+  Hint Unfold t: unalias.
+  Definition top: t := Blk H.top.
+  Definition hierarchy x y :=
+    match x, y with
+    | Blk a, Blk b   => H.hierarchy a b
+    | Blk a, Loc b _ => a = b \/ H.hierarchy a b
+    | _, _ => False
+    end.
+  Definition parent x :=
+    match x with
+    | Loc b _ => Some (Blk b)
+    | Blk b   =>
+      match H.parent b with
+      | Some pb => Some (Blk pb)
+      | None    => None
+      end
+    end.
+  Definition measure x :=
+    (
+    match x with
+    | Loc b _ => 1 + H.measure b
+    | Blk b   => H.measure b
+    end
+    )%nat.
+  Definition eq_dec: forall (x y: t), {eq x y} + {~ eq x y}.
+  Proof.
+    repeat decide equality; try apply H.eq_dec; apply Int.eq_dec.
+  Defined.
+  Definition hierarchy_dec: forall x y, {hierarchy x y} + {~ hierarchy x y}.
+  Proof.
+    intros. destruct x, y; auto. apply H.hierarchy_dec. destruct (H.eq_dec t0 t1).
+    subst. left. simpl. auto.
+    simpl. destruct (H.hierarchy_dec t0 t1); intuition.
+  Defined.
+  Theorem top_spec: forall x, x <> top -> hierarchy top x.
+  Proof.
+    intros. simpl in *. destruct x. unfold top in H.
+    apply H.top_spec. congruence.
+    destruct (H.eq_dec H.top t0). auto. right. apply H.top_spec. auto.
+  Qed.
+  Theorem parent_measure: forall x px, parent x = Some px -> measure x = S (measure px).
+  Proof.
+    intros. destruct x; simpl in *. destruct (H.parent t0) as []_eqn; inv H.
+    apply H.parent_measure. auto.
+    inv H. auto.
+  Qed.
+End OptIntH.
+
+Module AbsPH := OptIntH(AbsBH).
+Module AbsPO := HtoO(AbsPH).
+
+Module OptIntOT (OT: OrderedType) <: OrderedType.
+  Definition t := @optint OT.t.
+  Definition eq (x y: t): Prop :=
+    match x, y with
+    | Blk a,   Blk b   => OT.eq a b
+    | Loc a x, Loc b y => OT.eq a b /\ x = y
+    | _,       _       => False
+    end.
+  Definition eq_equiv := @eq_equivalence.
+  Definition eq_refl: forall (x: t), eq x x.
+  Proof.
+    intros. destruct x. apply OT.eq_refl. split; auto.
+  Defined.
+  Theorem eq_sym: forall x y, eq x y -> eq y x.
+  Proof.
+    intros. destruct x, y; simpl in *; intuition; auto.
+  Qed.
+  Theorem eq_trans: forall (x y z: t), eq x y -> eq y z -> eq x z.
+  Proof.
+    destruct x, y, z; simpl in *; intuition; subst; auto; eapply OT.eq_trans; eauto.
+  Qed.
+  Definition eq_dec : forall x y, {eq x y}+{~eq x y}.
+  Proof.
+    unfold eq. destruct x, y; repeat decide equality; auto. apply OT.eq_dec.
+    pose proof (OT.eq_dec t0 t1). pose proof (Int.eq_dec i i0). intuition.
+  Defined.
+  Definition lt (x y: t) : Prop :=
+    match x, y with
+    | Blk a,   Blk b   => OT.lt a b
+    | Loc a x, Loc b y => OT.lt a b \/ (OT.eq a b /\ Int.lt x y = true)
+    | Loc _ _, Blk _   => True
+    | Blk _,   Loc _ _ => False
+    end.
+  Theorem lt_trans : forall x y z, lt x y -> lt y z -> lt x z.
+  Proof.
+    intros. destruct x, y, z; simpl in *; intuition; subst; auto.
+    eapply OT.lt_trans; eauto.
+    left. eapply OT.lt_trans; eauto.
+    left. destruct (OT.compare t0 t2). auto.
+    exfalso. eapply OT.lt_not_eq; eauto.
+    exfalso. eapply OT.lt_not_eq. eapply OT.lt_trans; eauto. apply OT.eq_sym. auto.
+    left. destruct (OT.compare t0 t2). auto.
+    exfalso. eapply OT.lt_not_eq; eauto.
+    exfalso. eapply OT.lt_not_eq. apply OT.lt_trans with (y:=t2); eauto. apply OT.eq_sym.
+    auto.
+    right. split. eapply OT.eq_trans; eauto. unfold Int.lt in *. repeat destruct zlt; auto.
+    omegaContradiction.
+  Qed.
+  Theorem lt_not_eq : forall x y : t, lt x y -> ~ eq x y.
+  Proof.
+    destruct x, y; simpl in *; intuition; try solve [eapply OT.lt_not_eq; eauto].
+    subst. unfold Int.lt in *. destruct zlt. omega. congruence.
+  Qed.
+  Definition compare : forall x y : t, Compare lt eq x y.
+  Proof.
+    intros. unfold lt. destruct x, y.
+    destruct (OT.compare t0 t1). apply LT. auto. apply EQ. auto. apply GT. auto.
+    apply GT. auto.
+    apply LT. auto.
+    destruct (OT.compare t0 t1). apply LT. auto.
+    destruct (Int.lt i i0) as []_eqn.
+    apply LT. right. split. apply e. auto.
+    destruct (Int.eq_dec i i0).
+    subst. apply EQ. simpl. auto.
+    apply GT. right. split. auto. unfold Int.lt in *. repeat (destruct zlt); auto.
+    assert (SEQ: Int.signed i = Int.signed i0) by omega.
+    apply (f_equal Int.repr) in SEQ. setoid_rewrite Int.repr_signed in SEQ. contradiction.
+    apply GT. auto.
+  Defined.
+End OptIntOT.
+
+Module AbsPOT := OptIntOT(AbsBOT).
+
+Ltac crunch_hierarchy :=
+  unfold AbsPH.t, AbsBH.t in *;
+  simpl in *;
+  try discriminate; try tauto;
+  match goal with
+  | b: absb |- _ => destruct b; crunch_hierarchy
+  | b: absb' |- _ => destruct b; crunch_hierarchy
+  | o: option _ |- _ => destruct o; crunch_hierarchy
+  | p: optint |- _ => destruct p; crunch_hierarchy
+  | H: Some _ = Some _ |- _ => inv H; crunch_hierarchy
+  | H: _ \/ _ |- _ => destruct H; crunch_hierarchy
+  | |- _ => idtac
+  end.
+
+Module PTSet
+  <: HSet(AbsPH)
+  <: SEMILATTICE_WITH_TOP.
+  Module AbsPSet := FSetAVL.Make AbsPOT.
+  Module F := FSetFacts.WFacts_fun AbsPOT AbsPSet.
+  Definition t := AbsPSet.t.
+  Definition add := AbsPSet.add.
+  Function In (x: AbsPH.t) (s: t) {measure AbsPH.measure x}: Prop :=
+    match AbsPH.parent x with
+    | Some px => AbsPSet.In x s \/ In px s
+    | None    => AbsPSet.In x s
+    end.
+  Proof.
+    intros. setoid_rewrite AbsPH.parent_measure at 2; eauto.
+  Qed.
+  Definition mem x s : {In x s} + {~In x s}.
+  Proof.
+    functional induction (In x s).
+    destruct IHP. auto.
+    destruct (AbsPSet.mem x s) as []_eqn.
+    apply F.mem_iff in Heqb. auto. apply F.not_mem_iff in Heqb. tauto.
+    destruct (AbsPSet.mem x s) as []_eqn.
+    apply F.mem_iff in Heqb. auto. apply F.not_mem_iff in Heqb. tauto.
+  Defined.
+  Definition bot := AbsPSet.empty.
+  Theorem In_add_same: forall x s, In x (add x s).
+  Proof.
+    intros. remember (add x s). functional induction (In x t0).
+    left. apply F.add_iff. destruct x; auto.
+    apply F.add_iff. destruct x; auto.
+  Qed.
+  Theorem In_add_hierarchy: forall x y,
+    AbsPH.hierarchy x y -> forall s, In y (add x s).
+  Proof.
+    intros. remember (add x s). functional induction (In y t0).
+    crunch_hierarchy; right; apply In_add_same.
+    crunch_hierarchy.
+  Qed.
+  Definition eq (s1 s2: t): Prop :=
+    forall x, In x s1 <-> In x s2.
+  Theorem eq_refl: forall x, eq x x.
+  Proof.
+    split; auto.
+  Qed.
+  Theorem eq_sym: forall x y, eq x y -> eq y x.
+  Proof.
+    split; specialize (H x0); destruct H; auto.
+  Qed.
+  Theorem eq_trans: forall x y z, eq x y -> eq y z -> eq x z.
+  Proof.
+    split; specialize (H x0); destruct H; specialize (H0 x0); destruct H0; auto.
+  Qed.
+  Definition beq: t -> t -> bool := AbsPSet.equal.
+  Lemma In_equiv:
+    forall x s,
+      In x s <->
+      AbsPSet.In x s \/
+      (exists px, AbsPH.parent x = Some px /\ In px s).
+  Proof.
+    split; intros.
+    functional induction (In x s).
+    destruct H; auto. right. exists px. auto.
+    auto.
+    functional induction (In x s).
+    destruct H; auto. destruct H as [px' [A B]]. rewrite A in e; inv e. auto.
+    destruct H; auto. destruct H as [px' [A B]]. rewrite A in e; inv e.
+  Qed.
+  Theorem In_add_already: forall x y s, In x s -> In x (add y s).
+  Proof.
+    intros.
+    apply In_equiv in H. apply In_equiv. intuition.
+    left. apply F.add_iff. auto.
+    right. destruct H0 as [px]. exists px. intuition.
+    apply In_equiv in H1. apply In_equiv. intuition.
+    left. apply F.add_iff. auto.
+    right. destruct H as [ppx]. exists ppx. intuition.
+    apply In_equiv in H2. apply In_equiv. intuition.
+    left. apply F.add_iff. auto.
+    right. destruct H as [pppx]. exists pppx. intuition.
+    apply In_equiv in H3. apply In_equiv. intuition.
+    left. apply F.add_iff. auto.
+    right. destruct H as [ppppx]. exfalso. intuition. crunch_hierarchy.
+  Qed.
+  Definition beq_correct: forall x y, beq x y = true -> eq x y.
+  Proof.
+    split; intros.
+    apply F.equal_iff in H. unfold AbsPSet.Equal in H.
+    functional induction (In x0 y).
+    apply In_equiv in H0.
+    destruct H0. left. apply H. apply H0.
+    destruct H0 as [px' [A B]]. rewrite A in e; inv e. right. auto.
+    apply In_equiv in H0. destruct H0.
+    apply H. apply H0.
+    destruct H0 as [px' [A B]]. rewrite A in e; inv e.
+    apply F.equal_iff in H. unfold AbsPSet.Equal in H.
+    functional induction (In x0 x).
+    apply In_equiv in H0.
+    destruct H0. left. apply H. apply H0.
+    destruct H0 as [px' [A B]]. rewrite A in e; inv e. right. auto.
+    apply In_equiv in H0. destruct H0.
+    apply H. apply H0.
+    destruct H0 as [px' [A B]]. rewrite A in e; inv e.
+  Qed.
+  Definition ge (s1 s2: t): Prop := forall x, In x s2 -> In x s1.
+  Theorem ge_refl: forall x y, eq x y -> ge x y.
+  Proof.
+    repeat intro. specialize (H x0). tauto.
+  Qed.
+  Theorem ge_trans: forall x y z, ge x y -> ge y z -> ge x z.
+  Proof.
+    repeat intro. specialize (H x0). specialize (H0 x0). tauto.
+  Qed.
+  Theorem ge_bot: forall x, ge x bot.
+  Proof.
+    repeat intro. remember bot. functional induction (In x0 t0).
+    destruct H. inv H. apply In_equiv. right. exists px. auto.
+    inv H.
+  Qed.
+  Definition lub (s: t) (s': t): t :=
+    let s'' := AbsPSet.union s s' in
+    AbsPSet.filter
+      (fun x =>
+        negb (AbsPSet.exists_ (AbsPH.hierarchy_dec x) s'')
+      )
+      s''.
+  Hypothesis ge_lub_left: forall x y, ge (lub x y) x.
+  Hypothesis ge_lub_right: forall x y, ge (lub x y) y.
+  Definition top := add AbsPH.top AbsPSet.empty.
+  Axiom ge_top: forall x, ge top x.
+  Definition singleton x := add x bot.
+  Axiom In_singleton: forall x, In x (singleton x).
+  Axiom In_singleton_hierarchy: forall x y,
+    AbsPH.hierarchy x y -> In y (singleton x).
+  Axiom not_In_bot: forall x, ~ In x bot.
+  Axiom In_top: forall x, In x top.
+  Axiom ge_top_eq_top: forall x, ge x top <-> eq x top.
+  Axiom top_ge: forall x, ge top x.
+  Opaque mem In beq ge lub bot top.
+  Hint Resolve In_add_same In_add_hierarchy eq_refl eq_sym eq_trans beq_correct
+    ge_refl ge_trans ge_bot ge_lub_left ge_lub_right In_singleton
+    In_singleton_hierarchy not_In_bot ge_top In_top ge_top_eq_top top_ge: ptset.
+End PTSet.
+
+(* Registers *)
+
+Module ROT <: OrderedType.
+  Definition t := reg.
+  Definition eq := @eq t.
+  Definition eq_refl := @refl_equal t.
+  Definition eq_sym := @sym_eq t.
+  Definition eq_trans := @trans_eq t.
+  Definition eq_dec := peq.
+  Definition lt := Plt.
+  Definition lt_trans := Plt_trans.
+  Theorem lt_not_eq : forall x y : t, lt x y -> ~ eq x y.
+  Proof.
+    repeat intro. inv H0. eapply Plt_strict. apply H.
+  Qed.
+  Definition compare : forall x y : t, Compare lt eq x y.
+  Proof.
+    intros. destruct (peq x y).
+    apply EQ. auto.
+    destruct (plt x y).
+    apply LT. auto. apply GT. destruct (plt y x). auto.
+    exfalso. unfold Plt in *. zify. omega.
+  Defined.
+End ROT.
+
+Module NaiveMergeStrategy (KEY: OrderedType) (VAL: SEMILATTICE)
+  <: MergeStrategy(KEY)(VAL).
+  Definition f (k: KEY.t) o1 o2 :=
+    match o1, o2 with
+    | None, None => None
+    | Some s, None | None, Some s => Some s
+    | Some s1, Some s2 => Some (VAL.lub s1 s2)
+    end.
+  Theorem f_compat:
+    forall x x' o1 o2,
+      KEY.eq x x' -> f x o1 o2 = f x' o1 o2.
+  Proof.
+    auto.
+  Qed.
+End NaiveMergeStrategy.
+
+Module RMapMergeStrategy := NaiveMergeStrategy(ROT)(PTSet).
+Module RMapWithoutTop := MapSemiLattice(ROT)(PTSet)(RMapMergeStrategy).
+
+Module RMap <: SEMILATTICE_WITH_TOP.
+  Module L := SemiLatticeToLattice(RMapWithoutTop).
+  Include L.
+  (* get should be like find, but wrapping the option type away *)
+  Definition get (k: ROT.t) (rmap: t): PTSet.t :=
+    match rmap with
+    | Top        => PTSet.top
+    | Some rmap' =>
+      match RMapWithoutTop.M.find k rmap' with
+      | None   => PTSet.bot
+      | Some s => s
+      end
+    end.
+
+  Definition add (r: ROT.t) (s: PTSet.t) (rmap: t): t :=
+    match rmap with
+    | Top        => Top
+    | Some rmap' => Some (RMapWithoutTop.M.add r s rmap')
+    end.
+
+  (*Parameter set: ROT.t -> PTSet.t -> t -> t.*)
+
+  Theorem get_ge: forall rmap rmap',
+    ge rmap rmap' ->
+    (forall k, PTSet.ge (RMap.get k rmap) (RMap.get k rmap')).
+  Proof.
+    intros. unfold get. destruct rmap, rmap'; auto with ptset.
+    specialize (H k).
+    destruct (RMapWithoutTop.M.find k t0);
+    destruct (RMapWithoutTop.M.find k t1);
+    auto with ptset.
+  Qed.
+  Axiom get_add_same: forall k v m, PTSet.ge (get k (add k v m)) v.
+  Axiom get_add: forall x y s m, PTSet.ge (get x (add y s m)) (get x m).
+  Axiom ge_add: forall k v m, ge (add k v m) m.
+  Axiom get_top: forall k, PTSet.ge (get k top) PTSet.top.
+  Global Opaque eq ge bot get add (*set*).
+End RMap.
+
+(* Memory *)
+
+Module AbsPOMap (L: SEMILATTICE_WITH_TOP)
+  <: OMap(AbsPO)(L)
+  <: SEMILATTICE_WITH_TOP.
+  Module AbsPOMapMergeStrategy :=
+    NaiveMergeStrategy(AbsPOT)(L). (* won't use it anyway *)
+  Module MSL := MapSemiLattice(AbsPOT)(L)(AbsPOMapMergeStrategy).
+  Module LAT := SemiLatticeToLattice(MSL).
+  Include LAT.
+
+  Function get_rec (k: AbsPO.t) (m: MSL.t) {measure AbsPO.measure k}: L.t :=
+    match MSL.M.find k m with
+    | Some s => s
+    | None   =>
+      match AbsPO.parent k with
+      | None   => L.bot
+      | Some p => get_rec p m
+      end
+    end.
+  Proof.
+    intros. rewrite (AbsPH.parent_measure k p teq0). auto.
+  Qed.
+
+  Definition get (k: AbsPO.t) (m: t): L.t :=
+    match m with
+    | Top    => L.top
+    | Some m => get_rec k m
+    end.
+
+  Definition lub_on_overlap (key: AbsPO.t) (val: L.t) (k: AbsPO.t) (v: L.t)
+    : L.t :=
+    if AbsPO.overlap_dec key k then L.lub v val else v.
+
+  Definition add_overlap key val m :=
+    MSL.M.mapi (lub_on_overlap key val) m.
+
+  Definition add (k: AbsPO.t) (v: L.t) (m: t): t :=
+    match m with
+    | Top    => Top
+    | Some m =>
+      Some (MSL.M.add k (L.lub v (get k (Some m))) (add_overlap k v m))
+    end.
+
+  (*Parameter set: AbsPO.t -> L.t -> t -> t.*)
+  Axiom get_add_same: forall k s m, L.ge (get k (add k s m)) s.
+  Axiom get_add: forall x y s m, L.ge (get x (add y s m)) (get x m).
+  Axiom get_add_overlap: forall x y s m,
+    AbsPO.overlap x y ->
+    L.ge (get x (add y s m)) s.
+  (*
+  Axiom get_set_same: forall k s m, L.ge (get k (set k s m)) s.
+  Axiom get_set_other: forall x y s m, L.ge (get x (set y s m)) (get x m).
+  *)
+  (* Additional lemmas *)
+  Theorem get_eq: forall mmap mmap',
+    eq mmap mmap' ->
+    (forall k, L.eq (get k mmap) (get k mmap')).
+  Proof.
+    intros. destruct mmap, mmap'; simpl in *.
+  Admitted.
+  Axiom get_ge: forall mmap mmap',
+    ge mmap mmap' ->
+    (forall k, L.ge (get k mmap) (get k mmap')).
+  Axiom get_top: forall k, L.ge (get k top) L.top.
+  Axiom get_eq_top: forall mmap,
+    eq mmap top ->
+    (forall k, L.ge (get k mmap) L.top).
+  Global Opaque eq ge bot get add (*set*) top.
+End AbsPOMap.
+
+Module MMap <: SEMILATTICE.
+  Module APOM := AbsPOMap(PTSet).
+  Include APOM.
+  Hint Resolve get_add_same get_add get_add_overlap
+  (*get_set_same get_set_other*)
+    get_eq get_ge get_top get_eq_top: mmap.
+End MMap.
+
+(* Result *)
+
+Module Result <: SEMILATTICE.
+  Module R := ProductSemiLattice(RMap)(MMap).
+  Include R.
+  Definition top := (RMap.top, MMap.top).
+End Result.
+
+Lemma fold_left_preserves_prop:
+  forall S F (P: S -> Prop) (f: S -> F -> S) l s,
+    P s ->
+    (forall x y, P x -> P (f x y)) ->
+    P (fold_left f l s).
+Proof.
+  induction l; simpl; auto.
+Qed.
+
+Lemma fold_left_adds_prop:
+  forall E S (e: E) (P: S -> Prop) (f: S -> E -> S) l s0 eq',
+    InA eq' e l ->
+    (forall x y, eq' x y -> x = y) ->
+    (forall x, P (f x e)) ->
+    (forall x y, P x -> P (f x y)) ->
+    P (fold_left f l s0).
+Proof.
+  induction l; intros.
+  inv H.
+  inv H. apply H0 in H4. subst.
+  simpl. apply fold_left_preserves_prop; auto.
+  eapply IHl; eauto.
+Qed.
+
+(* Transfer function *)
+Definition shift_offset (s: PTSet.t) (o: Int.int): PTSet.t :=
+  PTSet.AbsPSet.fold
+    (fun x saccu =>
+      match x with
+      | Blk _    => PTSet.AbsPSet.add x saccu
+      | Loc b o' => PTSet.AbsPSet.add (Loc b (Int.add o o')) saccu
+      end
+    )
+    s
+    PTSet.AbsPSet.empty.
+Definition unknown_offset (s: PTSet.t): PTSet.t :=
+  PTSet.AbsPSet.fold
+    (fun x saccu =>
+      match x with
+      | Blk _   => PTSet.AbsPSet.add x saccu
+      | Loc b o => PTSet.AbsPSet.add (Blk b) saccu
+      end
+    )
+    s
+    PTSet.AbsPSet.empty.
+
+Theorem In_unknown_offset_block_of_loc:
+  forall b o s
+    (IN: PTSet.AbsPSet.In (Loc b o) s),
+    PTSet.In (Blk b) (unknown_offset s).
+Proof.
+  intros. unfold unknown_offset. rewrite PTSet.AbsPSet.fold_1.
+  eapply fold_left_adds_prop.
+  apply PTSet.F.elements_iff. eauto.
+  intros. destruct x, y; subst; try (intuition; congruence).
+  simpl. apply PTSet.In_add_same.
+  intros.
+  apply PTSet.In_equiv in H. intuition; apply PTSet.In_equiv.
+  left; destruct y; apply PTSet.F.add_iff; right; auto.
+  right. destruct H0 as [px]. exists px. intuition.
+  apply PTSet.In_equiv in H1. intuition; apply PTSet.In_equiv.
+  left; destruct y; apply PTSet.F.add_iff; right; auto.
+  right. destruct H as [px']. exists px'. intuition.
+  apply PTSet.In_equiv in H2. intuition; apply PTSet.In_equiv.
+  left; destruct y; apply PTSet.F.add_iff; right; auto.
+  exfalso.
+  destruct H as [px'']. intuition. crunch_hierarchy.
+Qed.
+
+Lemma In_unknown_offset_same_aux:
+  forall p s
+    (IN: PTSet.AbsPSet.In p s),
+    PTSet.In p (unknown_offset s).
+Proof.
+  intros. apply PTSet.In_equiv. destruct p.
+  left. unfold unknown_offset. rewrite PTSet.AbsPSet.fold_1.
+  eapply fold_left_adds_prop.
+  apply PTSet.F.elements_iff. eauto.
+  intros. destruct x, y; subst; try (intuition; congruence).
+  simpl. intros. apply PTSet.F.add_iff. auto.
+  intros. destruct y; apply PTSet.F.add_iff; right; auto.
+  right. exists (Blk a). intuition. apply PTSet.In_equiv. left.
+  unfold unknown_offset. rewrite PTSet.AbsPSet.fold_1.
+  eapply fold_left_adds_prop.
+  apply PTSet.F.elements_iff. eauto.
+  intros. destruct x, y; subst; try (intuition; congruence).
+  simpl. intros. apply PTSet.F.add_iff. auto.
+  intros. destruct y; apply PTSet.F.add_iff; right; auto.
+Qed.
+
+Theorem In_unknown_offset_same:
+  forall p s
+    (IN: PTSet.In p s),
+    PTSet.In p (unknown_offset s).
+Proof.
+  intros.
+  apply PTSet.In_equiv in IN. intuition.
+  apply In_unknown_offset_same_aux. auto.
+  destruct H as [pp]. intuition. apply PTSet.In_equiv. right. exists pp.
+  intuition.
+  apply PTSet.In_equiv in H1. intuition.
+  apply In_unknown_offset_same_aux. auto.
+  destruct H as [ppp]. intuition. apply PTSet.In_equiv. right. exists ppp.
+  intuition.
+  apply PTSet.In_equiv in H2. intuition.
+  apply In_unknown_offset_same_aux. auto.
+  destruct H as [pppp]. intuition. apply PTSet.In_equiv. right. exists pppp.
+  intuition.
+  apply PTSet.In_equiv in H3. intuition.
+  apply In_unknown_offset_same_aux. auto.
+  destruct H as [ppppp]. intuition.
+  crunch_hierarchy.
+Qed.
+
+(*
+Check MMap.MSL.M.fold.
+=>
+Anomaly: uncaught exception Failure "Cannot print a global reference".
+Please report.
+*)
+
+Definition image_of_ptset (s: PTSet.t) (m: MMap.t): PTSet.t :=
+  PTSet.AbsPSet.fold
+    (fun p saccu => PTSet.lub (MMap.get p m) saccu)
+    s
+    PTSet.bot.
+
+Definition add_ptset_to_image (sadd: PTSet.t) (smod: PTSet.t) (m: MMap.t)
+  : MMap.t :=
+  PTSet.AbsPSet.fold (fun k maccu => MMap.add k sadd maccu) smod m.
+
+Definition addr_image addr args rmap :=
+  match addr, args with
+    | Aindexed o, r::nil             =>
+      Some (shift_offset (RMap.get r rmap) o)
+    | Aindexed2 _, r1::r2::nil       =>
+      Some (PTSet.lub
+        (unknown_offset (RMap.get r1 rmap))
+        (unknown_offset (RMap.get r2 rmap))
+      )
+    | Ascaled _ _, _::nil            => Some PTSet.bot
+    | Aindexed2scaled _ _, r::_::nil =>
+      Some (unknown_offset (RMap.get r rmap))
+    | Aglobal i o, nil               =>
+      Some (PTSet.singleton (Loc (Just (Globals (Just i))) o))
+    | Abased i _, _::nil
+    | Abasedscaled _ i _, _::nil     =>
+      Some (PTSet.singleton (Blk (Just (Globals (Just i)))))
+    | Ainstack o, nil                =>
+      Some (PTSet.singleton (Loc (Just Stack) o))
+    | _, _                           => None
+  end.
+
+Definition transf_op op args dst rmap :=
+  match op with
+    | Olea addr =>
+      match addr_image addr args rmap with
+        | None   => rmap (*!*)
+        | Some s => RMap.add dst s rmap
+      end
+    | Omove     =>
+      match args with
+        | r::nil => RMap.add dst (RMap.get r rmap) rmap
+        | _      => rmap (*!*)
+      end
+    | Osub      =>
+      match args with
+        | r::_::nil => RMap.add dst (unknown_offset (RMap.get r rmap)) rmap
+        | _         => rmap (*!*)
+      end
+    | _         => rmap
+  end.
+
+Definition transf_builtin ef args dst n (result: Result.t) :=
+  let (rmap, mmap) := result in
+  match ef with
+  | EF_external _ sg =>
+    (RMap.add dst (PTSet.singleton (Blk (Just (Globals All)))) rmap, mmap)
+  | EF_builtin _ sg  =>
+    (RMap.add dst (PTSet.singleton (Blk (Just (Globals All)))) rmap, mmap)
+  | EF_vload chunk   => (RMap.add dst PTSet.top rmap, mmap)
+  | EF_vstore chunk  =>
+    match args with
+    | r1 :: r2 :: nil =>
+      (rmap, add_ptset_to_image (RMap.get r2 rmap) (RMap.get r1 rmap) mmap)
+    | _               => result
+    end
+  | EF_malloc        =>
+    (RMap.add dst (PTSet.singleton (Loc (Just (Allocs (Just n))) Int.zero)) rmap, mmap)
+  | EF_free          => result
+  | EF_memcpy _ _    =>
+    match args with
+    | rdst :: rsrc :: nil =>
+      (rmap, add_ptset_to_image PTSet.top (unknown_offset (RMap.get rdst rmap)) mmap)
+    | _                   => result (*!*)
+    end
+  | EF_annot _ _     => result
+  | EF_annot_val _ _ =>
+    match args with
+    | r1 :: nil => (RMap.add dst (RMap.get r1 rmap) rmap, mmap)
+    | _       => result (*!*)
+    end
+  | EF_vload_global _ _ _ => result (* TODO *)
+  | EF_vstore_global _ _ _ => result (* TODO *)
+  end.
+
+Definition transf c n (result: Result.t) :=
+  let (rmap, mmap) := result in
+  match c!n with
+  | Some instr =>
+    match instr with
+    | Inop _                          => result
+    | Iop op args dst succ            => (transf_op op args dst rmap, mmap)
+    | Iload chunk addr args dst succ  =>
+      match chunk with
+      | Mint32 =>
+        match addr_image addr args rmap with
+        | None   => result (*!*)
+        | Some s => (RMap.add dst (image_of_ptset s mmap) rmap, mmap)
+        end
+      | _ => (RMap.add dst PTSet.bot rmap, mmap)
+      end
+    | Istore chunk addr args src succ =>
+      match chunk with
+      | Mint32 =>
+        match addr_image addr args rmap with
+        | None      => result (*!*)
+        | Some sdst => (rmap, add_ptset_to_image (RMap.get src rmap) sdst mmap)
+        end
+      | _ => result
+      end
+    | Icall sign fn args dst succ     => (RMap.add dst PTSet.top rmap, MMap.top)
+    | Itailcall sign fn args          => (rmap, MMap.top)
+    | Ibuiltin ef args dst succ       => transf_builtin ef args dst n result
+    | Icond cond args ifso ifnot      => result
+    | Ijumptable arg tbl              => result
+    | Ireturn _                       => result
+    end
+  | None       => result
+  end.
+
+(* Kildall solver *)
+
+Module Solver := Dataflow_Solver(Result)(NodeSetForward).
+
+Definition coerce_solver (res: Solver.L.t): (RMap.t * MMap.t) := res.
+
+Definition add_reg_top rmap r := RMap.add r PTSet.top rmap.
+
+Definition entry_rmap l := fold_left add_reg_top l RMap.bot.
+
+Definition entry_mmap :=
+  MMap.add (Blk (Just (Globals All))) PTSet.top (
+  MMap.add (Blk (Just Other)) PTSet.top (
+  MMap.bot)).
+
+Definition entry_result l := (entry_rmap l, entry_mmap).
+
+Definition funanalysis f :=
+  Solver.fixpoint (successors f) (transf (fn_code f))
+  ((fn_entrypoint f, entry_result (fn_params f)) :: nil).
+
+Definition safe_funanalysis f :=
+  match funanalysis f with
+  | Some result => result
+  | None        => PMap.init Result.top
+  end.
+Hint Unfold safe_funanalysis: unalias.
+
+(* Proof invariant definitions *)
+
+Definition abstracter := block -> option absb.
+
+Definition valsat (v: val) (abs: abstracter) (s: PTSet.t) :=
+  match v with
+  | Vptr b o =>
+    match abs b with
+    | Some ab => PTSet.In (Loc ab o) s
+    | None    => PTSet.ge s PTSet.top (* equivalent to eq but easier in proofs *)
+    end
+  | _        => True
+  end.
+Hint Unfold valsat: unalias.
+
+Definition regsat (r: reg) (rs: regset) (abs: abstracter) (rmap: RMap.t) :=
+  valsat rs#r abs (RMap.get r rmap).
+Hint Unfold regsat: unalias.
+
+Definition memsat
+  (b: block) (o: Int.int) (m: mem) (abs: abstracter) (mmap: MMap.t)
+  :=
+  forall v
+    (LOAD: Mem.loadv Mint32 m (Vptr b o) = Some v)
+    ,
+    (match abs b with
+     | Some ab => valsat v abs (MMap.get (Loc ab o) mmap)
+     | None    => False
+     end).
+Hint Unfold memsat: unalias.
+
+Definition ok_abs_mem (abs: abstracter) (m: mem) :=
+  forall b, abs b <> None <-> Mem.valid_block m b.
+Hint Unfold ok_abs_mem : unalias.
+
+Definition ok_abs_genv (abs: abstracter) (ge: genv) :=
+  forall i b
+    (FIND: Genv.find_symbol ge i = Some b)
+    ,
+    abs b = Some (Just (Globals (Just i))).
+Hint Unfold ok_abs_genv : unalias.
+
+(* This is factored out to delay the instantiation of rmap, mmap in ok_stack *)
+Inductive ok_abs_result_stack f pc rs rret abs: Prop :=
+| ok_abs_result_stack_intro: forall rmap mmap
+  (RPC:  (safe_funanalysis f)#pc = (rmap, mmap))
+  (RSAT: forall r, regsat r rs abs rmap)
+  (RET:  PTSet.ge (RMap.get rret rmap) PTSet.top) (* same as eq, easier *)
+  (MTOP: MMap.eq mmap MMap.top)
+  ,
+  ok_abs_result_stack f pc rs rret abs.
+
+Inductive ok_stack (ge: genv) (b: block): list stackframe -> Prop :=
+| ok_stack_nil:
+  ok_stack ge b nil
+| ok_stack_cons: forall r f bsp pc rs stk abs
+  (STK:  ok_stack ge b stk)
+  (MEM:  forall b', abs b' <> None -> b' < b)
+  (GENV: ok_abs_genv abs ge)
+  (SP:   abs bsp = Some (Just Stack))
+  (RES:  ok_abs_result_stack f pc rs r abs)
+  ,
+  ok_stack ge b (Stackframe r f (Vptr bsp Int.zero) pc rs :: stk)
+.
+
+(* This is factored out to delay the instantiation of rmap, mmap in satisfy *)
+Inductive ok_abs_result f pc rs m abs: Prop :=
+| ok_abs_result_intro: forall rmap mmap
+  (RPC:  (safe_funanalysis f)#pc = (rmap, mmap))
+  (RSAT: forall r, regsat r rs abs rmap)
+  (MSAT: forall b o, memsat b o m abs mmap)
+  ,
+  ok_abs_result f pc rs m abs.
+
+Inductive satisfy (ge: genv) (abs: abstracter): state -> Prop :=
+| satisfy_state: forall cs f bsp pc rs m
+  (STK:  ok_stack ge (Mem.nextblock m) cs)
+  (MEM:  ok_abs_mem abs m)
+  (GENV: ok_abs_genv abs ge)
+  (SP:   abs bsp = Some (Just Stack))
+  (RES:  ok_abs_result f pc rs m abs)
+  ,
+  satisfy ge abs (State cs f (Vptr bsp Int.zero) pc rs m)
+| satisfy_callstate: forall cs f args m
+  (MEM:  ok_abs_mem abs m)
+  (STK:  ok_stack ge (Mem.nextblock m) cs)
+  (GENV: ok_abs_genv abs ge)
+  ,
+  satisfy ge abs (Callstate cs f args m)
+| satisfy_returnstate: forall cs v m
+  (MEM:  ok_abs_mem abs m)
+  (STK:  ok_stack ge (Mem.nextblock m) cs)
+  (GENV: ok_abs_genv abs ge)
+  ,
+  satisfy ge abs (Returnstate cs v m)
+.
+
+(* Lemmas *)
+
+Ltac regsat_intro rs r :=
+  match goal with
+  | H: Vptr _ _ = rs#r |- _ => apply symmetry in H; regsat_intro rs r
+  | R: (forall r, regsat r rs _ _),
+    H: rs#r = Vptr _ _ |- _ =>
+      let IN := fresh "IN" in
+      pose proof (R r) as IN; unfold regsat, valsat in IN; rewrite H in IN
+  end.
+
+Ltac crunch_eval :=
+  match goal with
+  | H: Val.add _ _ = _ |- _ => unfold Val.add in *; crunch_eval
+  | H: Val.mul _ _ = _ |- _ => unfold Val.mul in *; crunch_eval
+  | H: symbol_address _ _ _ = _ |- _ => unfold symbol_address in *; crunch_eval
+  | H: Vptr _ _ = Vptr _ _ |- _ => inv H; crunch_eval
+  | H: Some _ = None   |- _ => inv H
+  | H: None   = Some _ |- _ => inv H
+  | H: Some _ = Some _ |- _ => inv H; crunch_eval
+  | H: (match _##?args with | nil => _ | _::_ => _ end) = _ |- _ =>
+    destruct args; simpl in H; try solve [inv H]; crunch_eval
+  | H: (match ?rs#?r with
+        | Vundef => _ | Vint _ => _ | Vfloat _ => _ | Vptr _ _ => _
+        end) = _ |- _ =>
+    destruct rs#r as []_eqn; [ | | | regsat_intro rs r]; try solve [inv H]; crunch_eval
+  | H: (if ?cond then _ else _) = _ |- _ =>
+    destruct cond as []_eqn; try solve [inv H]; crunch_eval
+  | H: (match ?opt with | Some _ => _ | None   => _ end) = _ |- _ =>
+    destruct opt as []_eqn; try solve [inv H]; crunch_eval
+  | H: (match ?opt with | Some _ => _ | None => _ end) |- _ =>
+    destruct opt as []_eqn; try solve [congruence]; crunch_eval
+  | H: (match ?val with
+        | Vundef => _ | Vint _ => _ | Vfloat _ => _ | Vptr _ _ => _
+        end) = _ |- _ =>
+    destruct val as []_eqn; try solve [inv H]; crunch_eval
+  | a: addressing |- _          => destruct a; simpl in *; crunch_eval
+  (*| H: offset_sp ?sp _ = _ |- _ => unfold offset_sp in H; crunch_eval*)
+  | H: option_map _ _ = _ |- _  => unfold option_map in H; crunch_eval
+  | _ => idtac
+  end.
+
+Ltac merge :=
+  match goal with
+  | H: ?x = ?x |- _ => clear H; merge
+  | H: (_, _) = (_, _) |- _ => inv H; merge
+  | H1: ?a = None,
+    H2: ?b = None |- _ => idtac (* prevents a loop *)
+  | H1: ?x = ?a,
+    H2: ?x = ?b |- _ =>
+      rewrite H1 in H2; inv H2; merge
+  | H1: ?a = ?x,
+    H2: ?b = ?x |- _ =>
+      rewrite <- H1 in H2; inv H2; merge
+  | H1: ?x = ?a,
+    H2: ?b = ?x |- _ =>
+      rewrite H1 in H2; inv H2; merge
+  | |- _ => idtac
+  end.
+
+Lemma In_unknown_offset:
+  forall b o s
+    (IN: PTSet.In (Loc b o) s)
+    ,
+    (forall o', PTSet.In (Loc b o') (unknown_offset s)).
+Proof.
+  intros. remember (Loc b o) as lb. remember (Loc b o') as lb'.
+  remember (unknown_offset s) as uos.
+  functional induction (PTSet.In lb s); [ | crunch_hierarchy].
+  clear IHP. destruct IN.
+  functional induction (PTSet.In lb' uos); [ | crunch_hierarchy].
+  clear IHP.
+  assert (px = px0) by (crunch_hierarchy; auto); subst.
+  right. destruct px0; inv e. eapply In_unknown_offset_block_of_loc; eauto.
+  functional induction (PTSet.In lb' uos); [ | crunch_hierarchy].
+  clear IHP.
+  assert (px = px0) by (crunch_hierarchy; auto); subst.
+  right. eauto using In_unknown_offset_same.
+Qed.
+
+Lemma In_shift_offset:
+  forall b o s o' oshift
+    (IN: PTSet.In (Loc b o) s)
+    (SH: o' = Int.add o oshift)
+    ,
+    PTSet.In (Loc b o') (shift_offset s oshift).
+Proof.
+  intros. subst. rewrite Int.add_commut.
+  unfold shift_offset. rewrite PTSet.AbsPSet.fold_1.
+  apply PTSet.In_equiv in IN. intuition.
+  eapply fold_left_adds_prop.
+  apply PTSet.F.elements_iff. eauto.
+  intros. destruct x, y; subst; try (intuition; congruence).
+  simpl. apply PTSet.In_add_same.
+  intros. destruct y; apply PTSet.In_add_already; auto.
+
+  destruct H as [px]. simpl in *. intuition. inv H0.
+  apply PTSet.In_equiv in H1. intuition.
+  eapply fold_left_adds_prop.
+  apply PTSet.F.elements_iff. eauto.
+  intros. destruct x, y; subst; try (intuition; congruence).
+  simpl. apply PTSet.In_add_hierarchy. simpl. auto.
+  intros. destruct y; apply PTSet.In_add_already; auto.
+
+  destruct H as [px]. intuition.
+  apply PTSet.In_equiv in H1. intuition.
+  eapply fold_left_adds_prop.
+  apply PTSet.F.elements_iff. eauto.
+  intros. destruct x, y; subst; try (intuition; congruence).
+  intros. destruct px, b; inv H0. apply PTSet.In_add_hierarchy.
+  destruct a; simpl; auto; destruct o0; simpl; auto.
+  intros. destruct y; apply PTSet.In_add_already; auto.
+
+  destruct H as [ppx]. intuition.
+  apply PTSet.In_equiv in H2. intuition.
+  eapply fold_left_adds_prop.
+  apply PTSet.F.elements_iff. eauto.
+  intros. destruct x, y; subst; try (intuition; congruence).
+  intros. crunch_hierarchy; apply PTSet.In_add_hierarchy; simpl; auto.
+  intros. destruct y; apply PTSet.In_add_already; auto.
+
+  destruct H as [pppx]. intuition. exfalso. crunch_hierarchy.
+Qed.
+
+Lemma unknown_offset_top:
+  forall s
+    (GETOP: PTSet.ge s PTSet.top)
+    ,
+    PTSet.ge (unknown_offset s) PTSet.top.
+Proof.
+Admitted.
+
+Lemma shift_offset_top:
+  forall s
+    (GETOP: PTSet.ge s PTSet.top)
+    ,
+    (forall oshift, PTSet.ge (shift_offset s oshift) PTSet.top).
+Proof.
+Admitted.
+
+Lemma In_image_of_ptset:
+  forall x y mmap s,
+    PTSet.In x s ->
+    PTSet.In y (MMap.get x mmap) ->
+    PTSet.In y (image_of_ptset s mmap).
+Proof.
+Admitted.
+
+Lemma In_add_ptset_to_image:
+  forall x y sfrom sto mmap
+    (FROM: PTSet.In x sfrom)
+    (TO:   PTSet.In y sto)
+    ,
+    PTSet.In x (MMap.get y (add_ptset_to_image sfrom sto mmap)).
+Proof.
+Admitted.
+
+Lemma ge_add_ptset_to_image:
+  forall mmap s s',
+    MMap.ge (add_ptset_to_image s s' mmap) mmap.
+Proof.
+Admitted.
+
+Lemma addr_image_correct:
+  forall ge rs rmap abs addr args b o ab s bsp
+    (GENV: ok_abs_genv abs ge)
+    (SP:   abs bsp = Some (Just Stack))
+    (RSAT: forall r, regsat r rs abs rmap)
+    (EA:   eval_addressing ge (Vptr bsp Int.zero) addr rs##args = Some (Vptr b o))
+    (ABS:  abs b = Some ab)
+    (MPTA: addr_image addr args rmap = Some s)
+    ,
+    PTSet.In (Loc ab o) s.
+Proof.
+  intros.
+  crunch_eval; merge.
+  eapply In_shift_offset; eauto.
+  apply PTSet.ge_lub_right. eapply In_unknown_offset; eauto.
+  apply PTSet.ge_lub_left. eapply In_unknown_offset; eauto.
+  eapply In_unknown_offset; eauto.
+  specialize (GENV _ _ Heqo0). merge. apply PTSet.In_singleton.
+  specialize (GENV _ _ Heqo). merge. apply PTSet.In_singleton_hierarchy. compute; auto.
+  specialize (GENV _ _ Heqo0). merge. apply PTSet.In_singleton_hierarchy. compute; auto.
+  rewrite Int.add_zero_l. apply PTSet.In_singleton.
+Qed.
+
+Lemma regsat_ge1:
+  forall rs rmap abs rmap' r
+    (RSAT: regsat r rs abs rmap)
+    (GE:   RMap.ge rmap' rmap)
+    ,
+    regsat r rs abs rmap'.
+Proof.
+  intros. unalias. destruct (rs#r); auto. destruct (abs b).
+  destruct (abs b), rmap, rmap'; auto with ptset; try solve [eapply RMap.get_ge; eauto].
+  eapply PTSet.ge_trans; eauto. apply RMap.get_ge. auto.
+Qed.
+
+Lemma regsat_ge:
+  forall rs rmap abs rmap'
+    (RSAT: forall r, regsat r rs abs rmap)
+    (GE:   RMap.ge rmap' rmap)
+    ,
+    (forall r, regsat r rs abs rmap').
+Proof.
+  intros. eapply regsat_ge1; eauto.
+Qed.
+
+Lemma regsat_assign_not_vptr:
+  forall rs rmap abs v rdst
+    (RSAT: forall r, regsat r rs abs rmap)
+    (NPTR: match v with Vptr _ _ => False | _ => True end)
+    ,
+    (forall r, regsat r rs#rdst<-v abs rmap).
+Proof.
+  intros. specialize (RSAT r). unalias.
+  destruct (peq r rdst).
+  subst. rewrite Regmap.gss. destruct v; auto.
+  contradiction.
+  rewrite Regmap.gso; auto.
+Qed.
+
+Lemma regsat_assign_other:
+  forall r res v rmap abs rs
+    (RSAT:  forall r, regsat r rs abs rmap)
+    (OTHER: res <> r)
+    ,
+    regsat r rs#res<-v abs rmap.
+Proof.
+  intros. specialize (RSAT r). unalias. rewrite Regmap.gso; auto.
+Qed.
+
+Lemma regsat_top:
+  forall rs abs,
+    (forall r, regsat r rs abs RMap.top).
+Proof.
+  intros. unalias. destruct (rs#r) as []_eqn; auto. destruct (abs b) as []_eqn.
+  apply RMap.get_top. apply PTSet.In_top.
+  apply RMap.get_top.
+Qed.
+
+Lemma memsat_ge:
+  forall m abs mmap mmap'
+    (MSAT: forall b o, memsat b o m abs mmap)
+    (GE:   MMap.ge mmap' mmap)
+    ,
+    (forall b o, memsat b o m abs mmap').
+Proof.
+  repeat intro. unalias. specialize (MSAT _ _ _ LOAD).
+  destruct (abs b), v; auto. destruct (abs b0).
+  eapply MMap.get_ge; eauto.
+  eapply PTSet.ge_trans; eauto. apply MMap.get_ge. auto.
+Qed.
+
+Lemma load_valid_block:
+  forall chunk m b ofs v,
+    Mem.load chunk m b ofs = Some v ->
+    Mem.valid_block m b.
+Proof.
+  intros. eapply Mem.load_valid_access in H. eapply Mem.valid_access_implies in H.
+  eapply Mem.valid_access_valid_block in H. auto. constructor.
+Qed.
+
+Lemma memsat_top:
+  forall m abs
+    (OKAM: ok_abs_mem abs m)
+    ,
+    (forall b o, memsat b o m abs MMap.top).
+Proof.
+  unalias. intros. destruct (abs b) as []_eqn.
+  destruct v; auto. destruct (abs b0) as []_eqn.
+  apply MMap.get_top. apply PTSet.In_top.
+  apply MMap.get_top.
+  simpl in LOAD. apply load_valid_block in LOAD. apply OKAM in LOAD. contradiction.
+Qed.
+
+Lemma memsat_free:
+  forall m abs ptm bf lo hi m'
+    (MSAT: forall b o, memsat b o m abs ptm)
+    (FREE: Mem.free m bf lo hi = Some m')
+    ,
+    (forall b o, memsat b o m' abs ptm).
+Proof.
+  intros. unfold memsat, valsat in *. intros. specialize (MSAT b o v).
+  feed MSAT. simpl in *. erewrite Mem.load_free in LOAD. eauto. eauto.
+  destruct (zeq b bf); auto. subst. apply Mem.load_valid_access in LOAD.
+  eapply Mem.valid_access_free_inv_2 in LOAD; eauto.
+  auto.
+Qed.
+
+Lemma ok_abs_mem_store:
+  forall abs m chunk b o v m'
+    (OKAM: ok_abs_mem abs m)
+    (STOR: Mem.store chunk m b o v = Some m')
+    ,
+    ok_abs_mem abs m'.
+Proof.
+  unalias. split; intros.
+  eapply Mem.store_valid_block_1; eauto. apply OKAM. auto.
+  apply OKAM. eapply Mem.store_valid_block_2; eauto.
+Qed.
+
+Lemma ok_abs_mem_free:
+  forall abs m b o s m'
+    (OKAM: ok_abs_mem abs m)
+    (FREE: Mem.free m b o s = Some m')
+    ,
+    ok_abs_mem abs m'.
+Proof.
+  unalias. split; intros.
+  eapply Mem.valid_block_free_1; eauto. apply OKAM. auto.
+  apply OKAM. eapply Mem.valid_block_free_2; eauto.
+Qed.
+
+Lemma ok_abs_mem_storebytes:
+  forall abs m b o s m'
+    (OK: ok_abs_mem abs m)
+    (SB: Mem.storebytes m b o s = Some m')
+    ,
+    ok_abs_mem abs m'.
+Proof.
+  unalias; intros. specialize (OK b0). split; intros. apply OK in H.
+  eapply Mem.storebytes_valid_block_1; eauto. apply OK.
+  eapply Mem.storebytes_valid_block_2; eauto.
+Qed.
+
+Lemma ok_stack_incr:
+  forall stk ge b, ok_stack ge b stk -> forall b', b <= b' -> ok_stack ge b' stk.
+Proof.
+  induction 1; intros; econstructor; eauto. intros. specialize (MEM b'0 H1). omega.
+Qed.
+
+Lemma ok_stack_alloc:
+  forall stack ge m m' lo hi b,
+    ok_stack ge (Mem.nextblock m) stack ->
+    Mem.alloc m lo hi = (m', b) ->
+    ok_stack ge (Mem.nextblock m') stack.
+Proof.
+  intros. eapply ok_stack_incr; eauto.
+  setoid_rewrite Mem.nextblock_alloc at 2; eauto. omega.
+Qed.
+
+Lemma load_alloc_other':
+  forall m1 lo hi m2 b,
+    Mem.alloc m1 lo hi = (m2, b) ->
+    forall b' ofs chunk,
+    b <> b' ->
+    Mem.load chunk m2 b' ofs = Mem.load chunk m1 b' ofs.
+Proof.
+  intros. destruct (Mem.load chunk m1 b' ofs) as []_eqn. pose proof Heqo as L.
+  eapply Mem.load_valid_access in Heqo. eapply Mem.valid_access_implies in Heqo.
+  eapply Mem.valid_access_valid_block in Heqo. erewrite Mem.load_alloc_unchanged; eauto.
+  constructor. destruct (Mem.load chunk m2 b' ofs) as []_eqn; auto.
+  eapply Mem.load_valid_access in Heqo0. eapply Mem.valid_access_implies in Heqo0.
+  eapply Mem.valid_access_alloc_inv in Heqo0; eauto. destruct (eq_block b' b).
+  congruence. eapply Mem.valid_access_load in Heqo0. destruct Heqo0. congruence.
+  constructor.
+Qed.
+
+Lemma load_vptr_Mint32:
+  forall chunk m a b o
+    (LOAD: Mem.loadv chunk m a = Some (Vptr b o))
+    ,
+    chunk = Mint32.
+Proof.
+  intros. unfold Mem.loadv in LOAD. destruct a; try solve [inv LOAD].
+  apply Mem.load_result in LOAD. symmetry in LOAD. apply decode_val_pointer_inv in LOAD.
+  destruct LOAD. subst. auto.
+Qed.
+
+(* Theorems *)
+
+Theorem satisfy_init:
+  forall p st
+    (IS:   initial_state p st),
+    exists abs, satisfy (Genv.globalenv p) abs st.
+Proof.
+  intros. inv IS.
+  exists (fun b =>
+    if zlt b (Mem.nextblock m0)
+      then
+        match Genv.invert_symbol ge b with
+        | Some i => Some (Just (Globals (Just i)))
+        | None   => Some (Just Other)
+        end
+      else None
+  ).
+  constructor.
+  Case "ok_abs_mem".
+  split; intros; destruct (zlt b0 (Mem.nextblock m0)); auto. elim H3. auto.
+  destruct (Genv.invert_symbol); congruence.
+  Case "ok_stack".
+  constructor.
+  Case "ok_abs_genv".
+  unalias; intros. destruct (zlt b0 (Mem.nextblock m0)).
+  eapply Genv.find_invert_symbol in FIND. unfold ge. rewrite FIND. auto.
+  eapply Genv.find_symbol_not_fresh in FIND; eauto. contradiction.
+Qed.
+
+Theorem satisfy_step:
+  forall ge st t st' abs
+    (SAT:  satisfy ge abs st)
+    (STEP: step ge st t st')
+    ,
+    exists abs', satisfy ge abs' st'.
+Proof.
+  intros.
+  destruct st; destruct st'; try solve [inv STEP]; inv SAT; try inv RES.
+
+  Case "state -> state".
+  unfold safe_funanalysis in RPC. destruct (funanalysis f) as []_eqn.
+  SCase "Kildall terminated".
+  pose proof Heqo as FPS.
+  eapply Solver.fixpoint_solution with (n:=pc)(s:=pc0) in FPS;
+  [ |
+  unfold successors; unfold successors_list; rewrite PTree.gmap1;
+  inv STEP; rewrite H6; simpl; try destruct b; auto; eapply list_nth_z_in; eauto
+  ].
+  rewrite RPC in FPS. unfold Solver.L.ge in FPS.
+  destruct (t0#pc0) as [rmap'' mmap'']_eqn.
+  destruct (transf (fn_code f) pc (rmap, mmap)) as [rmap' mmap']_eqn.
+  destruct FPS as [RGE MGE].
+  inv STEP; unfold transf in Heqt0; rewrite H6 in Heqt0; inv Heqt0;
+  try solve [exists abs; constructor; auto; econstructor;
+    [unalias; rewrite Heqo; eauto | eapply regsat_ge; eauto | eapply memsat_ge; eauto]].
+  SSCase "Iop".
+  exists abs; constructor; auto.
+  SSSCase "ok_abs_result".
+  econstructor.
+  SSSSCase "result".
+  unfold safe_funanalysis. rewrite Heqo. eauto.
+  SSSSCase "regsat".
+  eapply regsat_ge; eauto.
+
+  Ltac regsat_tac :=
+    simpl in *;
+    match goal with
+    (* Easy case: same rs, higher rmap *)
+    | H: forall r, regsat r ?rs ?abs ?rmap
+      |- forall r, regsat r ?rs ?abs (RMap.add _ _ ?rmap) =>
+        eapply regsat_ge; [apply H | apply RMap.ge_add]
+    (* Simple cases: assigning something that is not a Vptr *)
+    | |- forall r, regsat r _#_<-(Vundef) _ _ =>
+      eapply regsat_assign_not_vptr; [ | auto]; regsat_tac
+    | |- forall r, regsat r _#_<-(Vint _) _ _ =>
+      eapply regsat_assign_not_vptr; [ | auto]; regsat_tac
+    | |- forall r, regsat r _#_<-(Vfloat _) _ _ =>
+      eapply regsat_assign_not_vptr; [ | auto]; regsat_tac
+
+    | |- forall r, regsat r _#_<-(if ?cond then _ else _) _ _ =>
+      destruct cond as []_eqn; regsat_tac
+    | H: context [if ?cond then _ else _] |- _ =>
+      destruct cond as []_eqn; try solve [inv H]; regsat_tac
+
+    | |- match ?foo with
+         | Vundef => _ | Vint _ => _ | Vfloat _ => _ | Vptr _ _ => _
+         end =>
+      destruct foo as []_eqn; regsat_tac
+
+    | |- context [?rs#?r] =>
+      destruct (rs#r) as []_eqn; simpl; try regsat_intro rs r; regsat_tac
+
+    | H: context [?rs#?r] |- _ =>
+      destruct (rs#r); simpl in H; inv H; try regsat_intro rs r; regsat_tac
+
+    | H: context [match ?rs ## ?args with | nil => _ | _ :: _ => _ end] |- _ =>
+      destruct args; simpl in H; try solve [inv H]; regsat_tac
+
+    | v: val
+      |- forall r, regsat r _#_<-?v _ _ =>
+      destruct v; regsat_tac
+
+    | |- match ?abs ?b with | Some _ => _ | None => _ end =>
+      destruct (abs b) as []_eqn; regsat_tac
+
+    | G: ok_abs_genv _ ?ge,
+      H: Genv.find_symbol ?ge _ = _
+      |- _ =>
+      specialize (G _ _ H); merge; regsat_tac
+
+    (* Almost done *)
+    | |- PTSet.In _ (RMap.get ?r (RMap.add ?r _ _)) =>
+      apply RMap.get_add_same; regsat_tac
+    | |- PTSet.ge (RMap.get ?r (RMap.add ?r _ _)) _ =>
+      eapply PTSet.ge_trans; [apply RMap.get_add_same | auto]; regsat_tac
+
+    | |- forall r, regsat r _#?res<-_ _ _ =>
+      let r := fresh "r" in intro r; destruct (peq res r);
+        [ subst; unfold regsat, valsat; rewrite Regmap.gss
+        | apply regsat_assign_other
+        ];
+        regsat_tac
+
+    | c: condition |- _ => destruct c; regsat_tac
+    | c: comparison |- _ => destruct c; regsat_tac
+
+    (* Non-recursive cases *)
+    | H: _ = Vptr _ _ |- _ => try solve [inv H]
+    | H: Vptr _ _ = _ |- _ => try solve [inv H]
+
+    | |- _ => auto
+    end.
+
+  destruct op; simpl in *; repeat (crunch_eval; regsat_tac).
+  SSSSSCase "Osub".
+  eapply In_unknown_offset; eauto.
+  apply unknown_offset_top; auto.
+  SSSSSCase "Olea Aindexed".
+  eapply In_shift_offset; eauto.
+  apply shift_offset_top; auto.
+  SSSSSCase "Olea Aindexed2".
+  apply PTSet.ge_lub_right. eapply In_unknown_offset; eauto.
+  eapply PTSet.ge_trans. apply PTSet.ge_lub_right. apply unknown_offset_top; auto.
+  apply PTSet.ge_lub_left. eapply In_unknown_offset; eauto.
+  eapply PTSet.ge_trans. apply PTSet.ge_lub_left. apply unknown_offset_top; auto.
+  SSSSSCase "Olea Aindexed2scaled".
+  eapply In_unknown_offset; eauto.
+  apply unknown_offset_top; auto.
+  SSSSSCase "Olea Aglobal".
+  apply PTSet.In_singleton.
+  SSSSSCase "Olea Abased".
+  apply PTSet.In_singleton_hierarchy. compute; auto.
+  SSSSSCase "Olea Abasedscaled".
+  apply PTSet.In_singleton_hierarchy. compute; auto.
+  SSSSSCase "Olea Ainstack".
+  rewrite Int.add_zero_l. apply PTSet.In_singleton.
+  SSSSCase "memsat".
+  eapply memsat_ge; eauto.
+  SSCase "Iload".
+  exists abs; constructor; auto.
+  SSSCase "ok_abs_result".
+  econstructor.
+  SSSSCase "result".
+  unfold safe_funanalysis. rewrite Heqo. eauto.
+  SSSSCase "regsat".
+  eapply regsat_ge; eauto.
+  destruct chunk; try solve [inv H0;
+    eapply regsat_assign_not_vptr;
+      [ eapply regsat_ge; [auto | apply RMap.ge_add]
+      | destruct v; auto; apply load_vptr_Mint32 in H14; congruence
+      ]
+  ].
+  intros. destruct (peq dst r).
+  SSSSSCase "r = dst".
+  subst. unfold regsat, valsat. rewrite Regmap.gss. destruct v; auto.
+  destruct a as [ | | |ba oa]; try solve [inv H14].
+  specialize (MSAT _ _ _ H14).
+  destruct (abs ba) as []_eqn; [|contradiction].
+  destruct (abs b) as []_eqn.
+  SSSSSSCase "abs b = Some".
+  crunch_eval; inv H0; apply RMap.get_add_same; eapply In_image_of_ptset;
+    eauto; merge.
+  eapply In_shift_offset; eauto.
+  apply PTSet.ge_lub_right. eapply In_unknown_offset; eauto.
+  apply PTSet.ge_lub_left. eapply In_unknown_offset; eauto.
+  eapply In_unknown_offset; eauto.
+  specialize (GENV _ _ Heqo2). merge. apply PTSet.In_singleton.
+  specialize (GENV _ _ Heqo1). merge. apply PTSet.In_singleton_hierarchy. compute; auto.
+  specialize (GENV _ _ Heqo1). merge. apply PTSet.In_singleton_hierarchy. compute; auto.
+  rewrite Int.add_zero_l. apply PTSet.In_singleton.
+  SSSSSSCase "abs b = None".
+  crunch_eval; inv H0; (
+  eapply PTSet.ge_trans;
+    [ apply RMap.get_add_same
+    | repeat intro; eapply In_image_of_ptset; [ | apply MSAT; apply PTSet.In_top]
+    ]); merge.
+  eapply In_shift_offset; eauto.
+  apply PTSet.ge_lub_right. eapply In_unknown_offset; eauto.
+  apply PTSet.ge_lub_left. eapply In_unknown_offset; eauto.
+  eapply In_unknown_offset; eauto.
+  apply unknown_offset_top; auto. apply PTSet.In_top.
+  specialize (GENV _ _ Heqo2). merge. apply PTSet.In_singleton.
+  specialize (GENV _ _ Heqo3). merge. apply PTSet.In_singleton_hierarchy. compute; auto.
+  specialize (GENV _ _ Heqo3). merge. apply PTSet.In_singleton_hierarchy. compute; auto.
+  merge. rewrite Int.add_zero_l. apply PTSet.In_singleton.
+  SSSSSCase "r <> dst".
+  eapply regsat_assign_other; eauto. destruct addr_image; inv H0; auto.
+  eapply regsat_ge; eauto. apply RMap.ge_add.
+  SSSSCase "memsat".
+  eapply memsat_ge; eauto. eapply MMap.ge_trans; eauto.
+  destruct chunk; try solve [inv H0; apply MMap.ge_refl; apply MMap.eq_refl].
+  destruct addr_image; inv H0; apply MMap.ge_refl; apply MMap.eq_refl.
+  SSCase "Istore".
+  assert (MGE': MMap.ge mmap' mmap) by (
+  destruct chunk; try solve [inv H0; apply MMap.ge_refl; apply MMap.eq_refl];
+  destruct addr_image; inv H0;
+    [ apply ge_add_ptset_to_image
+    | apply MMap.ge_refl; apply MMap.eq_refl
+    ]).
+  exists abs. destruct a; try solve [inv H14]. constructor; auto.
+  SSSCase "ok_stack".
+  erewrite Mem.nextblock_store; eauto.
+  SSSCase "ok_abs_mem".
+  eapply ok_abs_mem_store; eauto.
+  SSSCase "ok_abs_result".
+  econstructor.
+  SSSSCase "result".
+  unfold safe_funanalysis. rewrite Heqo. eauto.
+  SSSSCase "regsat".
+  eapply regsat_ge; eauto. eapply RMap.ge_trans; eauto. eapply RMap.ge_refl.
+  destruct chunk; try solve [inv H0; apply RMap.eq_refl].
+  destruct addr_image; inv H0; apply RMap.eq_refl.
+  SSSSCase "memsat".
+  eapply memsat_ge; eauto.
+  intros. specialize (MSAT b0 o). unfold memsat, valsat in *. intros.
+  pose proof (Mem.valid_access_load m Mint32 b0 (Int.unsigned o)) as LOAD'.
+  feed LOAD'. eapply Mem.store_valid_access_2; eauto. eapply Mem.load_valid_access; eauto.
+  destruct LOAD' as [v' LOAD']. specialize (MSAT _ LOAD').
+  destruct (zeq b b0).
+  SSSSSCase "Stored in b".
+  subst.
+  destruct (zlt (Int.unsigned i) (Int.unsigned o + size_chunk Mint32)).
+  destruct (zlt (Int.unsigned o) (Int.unsigned i + size_chunk chunk)).
+  SSSSSSCase "Overlapped offset o".
+  destruct (abs b0) as []_eqn; [|contradiction].
+  destruct v; auto. pose proof LOAD as LOAD''.
+  eapply Mem.load_pointer_store in LOAD; eauto.
+  intuition; try solve [omegaContradiction]. subst. simpl in *.
+  assert (i = o)
+    by (apply f_equal with (f:=Int.repr) in H5; rewrite Int.repr_unsigned in H5;
+      rewrite Int.repr_unsigned in H5; auto). subst. clear z z0 H5.
+  regsat_intro rs0 src.
+  destruct (addr_image addr args rmap) as []_eqn; [|crunch_eval]. inv H0.
+  eapply addr_image_correct in Heqo1; eauto.
+  destruct (abs b) as []_eqn.
+  SSSSSSSSCase "abs b = Some".
+  apply In_add_ptset_to_image; auto.
+  SSSSSSSSCase "abs b = None".
+  repeat intro. apply In_add_ptset_to_image; auto.
+  SSSSSSCase "Didn't overlap offset o".
+  simpl in LOAD.
+  erewrite Mem.load_store_other in LOAD; eauto; [|right; right; omega]. merge.
+  destruct (abs b0) as []_eqn; [|contradiction].
+  destruct v; auto.
+  destruct (abs b) as []_eqn.
+  SSSSSSSCase "abs b = Some".
+  eapply MMap.get_ge; eauto.
+  SSSSSSSCase "abs b = None".
+  eapply PTSet.ge_trans; eauto. apply MMap.get_ge; auto.
+  SSSSSSCase "Didn't overlap offset o, for another reason".
+  simpl in LOAD.
+  erewrite Mem.load_store_other in LOAD; eauto; [|right; left; omega]. merge.
+  destruct (abs b0) as []_eqn; [|contradiction].
+  destruct v; auto.
+  destruct (abs b) as []_eqn.
+  SSSSSSSCase "abs b = Some".
+  eapply MMap.get_ge; eauto.
+  SSSSSSSCase "abs b = None".
+  eapply PTSet.ge_trans; eauto. apply MMap.get_ge; auto.
+  SSSSSCase "Didn't store in b0".
+  simpl in LOAD. erewrite Mem.load_store_other in LOAD; eauto. merge.
+  destruct (abs b0) as []_eqn; [|contradiction].
+  destruct v; auto.
+  destruct (abs b1) as []_eqn.
+  SSSSSSCase "abs b1 = Some".
+  eapply MMap.get_ge; eauto.
+  SSSSSSCase "abs b1 = None".
+  eapply PTSet.ge_trans; eauto. apply MMap.get_ge; auto.
+  SSCase "Ibuiltin".
+  assert (RGE': RMap.ge rmap' rmap) by (
+  destruct ef; repeat (
+    try solve [inv H0; apply RMap.ge_add];
+    try solve [inv H0; apply RMap.ge_refl; apply RMap.eq_refl];
+    destruct args)).
+  assert (MGE': MMap.ge mmap' mmap) by (
+  destruct ef; repeat (
+    try solve [inv H0; apply ge_add_ptset_to_image];
+    try solve [inv H0; apply MMap.ge_refl; apply MMap.eq_refl];
+    destruct args)).
+  destruct ef; inv H13; merge.
+  SSSCase "EF_external".
+  exists abs. constructor; auto.
+  SSSSCase "ok_abs_result".
+  econstructor.
+  SSSSSCase "result".
+  unfold safe_funanalysis. rewrite Heqo. eauto.
+  SSSSSCase "regsat".
+  intros; destruct (peq res r); [subst | eapply regsat_assign_other; eauto;
+    eapply regsat_ge; [eauto | eapply RMap.ge_trans; eauto]].
+  unfold regsat, valsat. rewrite Regmap.gss. destruct v; auto.
+  inv H1. specialize (GENV _ _ H4). rewrite GENV.
+  eapply PTSet.ge_trans. apply RMap.get_ge; apply RGE. apply RMap.get_add_same.
+  apply PTSet.In_singleton_hierarchy. compute; auto.
+  SSSSSCase "memsat".
+  eapply memsat_ge; eauto.
+  SSSCase "EF_builtin".
+  exists abs. constructor; auto.
+  SSSSCase "ok_abs_result".
+  econstructor.
+  SSSSSCase "result".
+  unfold safe_funanalysis. rewrite Heqo. eauto.
+  SSSSSCase "regsat".
+  intros; destruct (peq res r); [subst | eapply regsat_assign_other; eauto;
+    eapply regsat_ge; [eauto | eapply RMap.ge_trans; eauto]].
+  unfold regsat, valsat. rewrite Regmap.gss. destruct v; auto.
+  inv H1. specialize (GENV _ _ H4). rewrite GENV.
+  eapply PTSet.ge_trans. apply RMap.get_ge; apply RGE. apply RMap.get_add_same.
+  apply PTSet.In_singleton_hierarchy. compute; auto.
+  SSSSSCase "memsat".
+  eapply memsat_ge; eauto.
+  SSSCase "EF_vload".
+  exists abs. constructor; auto.
+  SSSSCase "ok_abs_result".
+  econstructor.
+  SSSSSCase "result".
+  unfold safe_funanalysis. rewrite Heqo. eauto.
+  SSSSSCase "regsat".
+  intros; destruct (peq res r); [subst | eapply regsat_assign_other; eauto;
+    eapply regsat_ge; [eauto | eapply RMap.ge_trans; eauto]].
+  unfold regsat, valsat. rewrite Regmap.gss. destruct v; simpl; auto.
+  regsat_tac.
+  eapply RMap.get_ge. eauto. apply RMap.get_add_same. apply PTSet.In_top.
+  eapply PTSet.ge_trans. apply RMap.get_ge. eauto. apply RMap.get_add_same.
+  SSSSSCase "memsat".
+  eapply memsat_ge; eauto.
+  inv H1. (* Check whether the store is volatile *)
+  SSSCase "EF_vstore (volatile)".
+  exists abs. constructor; auto.
+  SSSSCase "ok_abs_result".
+  econstructor.
+  SSSSSCase "result".
+  unfold safe_funanalysis. rewrite Heqo. eauto.
+  SSSSSCase "regsat".
+  intros; destruct (peq res r); [subst | eapply regsat_assign_other; eauto;
+    eapply regsat_ge; [eauto | eapply RMap.ge_trans; eauto]].
+  unfold regsat, valsat. rewrite Regmap.gss. auto.
+  SSSSSCase "memsat".
+  eapply memsat_ge; eauto. eapply MMap.ge_trans; eauto.
+  SSSCase "EF_vstore (not volatile)".
+  exists abs. constructor; auto.
+  SSSSCase "ok_stack".
+  erewrite Mem.nextblock_store; eauto.
+  SSSSCase "ok_abs_mem".
+  eapply ok_abs_mem_store; eauto.
+  SSSSCase "ok_abs_result".
+  econstructor.
+  SSSSSCase "result".
+  unfold safe_funanalysis. rewrite Heqo. eauto.
+  SSSSSCase "regsat".
+  intros; destruct (peq res r); [subst | eapply regsat_assign_other; eauto;
+    eapply regsat_ge; [eauto | eapply RMap.ge_trans; eauto]].
+  unfold regsat, valsat. rewrite Regmap.gss. auto.
+  SSSSSCase "memsat".
+  eapply memsat_ge; eauto.
+  repeat (destruct args; try solve [inv H]). inv H. inv H0.
+  intros. specialize (MSAT b0 o). unfold memsat, valsat in *. intros.
+  pose proof (Mem.valid_access_load m Mint32 b0 (Int.unsigned o)) as LOAD'.
+  feed LOAD'. eapply Mem.store_valid_access_2; eauto. eapply Mem.load_valid_access; eauto.
+  destruct LOAD' as [v' LOAD']. specialize (MSAT _ LOAD').
+  destruct (zeq b b0).
+  SSSSSSCase "Stored in b".
+  subst.
+  destruct (zlt (Int.unsigned ofs) (Int.unsigned o + size_chunk Mint32)).
+  destruct (zlt (Int.unsigned o) (Int.unsigned ofs + size_chunk chunk)).
+  SSSSSSSCase "Overlapped offset o".
+  destruct (abs b0) as []_eqn; [|contradiction].
+  destruct v; auto. pose proof LOAD as LOAD''.
+  eapply Mem.load_pointer_store in LOAD; eauto.
+  intuition; try solve [omegaContradiction]. merge. subst. simpl in *.
+  assert (o = ofs)
+    by (apply f_equal with (f:=Int.repr) in H8; rewrite Int.repr_unsigned in H8;
+      rewrite Int.repr_unsigned in H8; auto). subst. clear z z0 H8.
+  regsat_intro rs r0. regsat_intro rs r. rewrite Heqo0 in IN0.
+  destruct (abs b) as []_eqn.
+  SSSSSSSSCase "abs b = Some".
+  apply In_add_ptset_to_image; auto.
+  SSSSSSSSCase "abs b = None".
+  eapply PTSet.ge_trans; eauto. repeat intro. apply In_add_ptset_to_image; auto.
+  SSSSSSSCase "Didn't overlap offset o".
+  simpl in LOAD.
+  erewrite Mem.load_store_other in LOAD; eauto; [|right; right; omega]. merge.
+  destruct (abs b0) as []_eqn; [|contradiction].
+  destruct v; auto.
+  destruct (abs b) as []_eqn.
+  SSSSSSSSCase "abs b = Some".
+  eapply MMap.get_ge; eauto.
+  SSSSSSSSCase "abs b = None".
+  eapply PTSet.ge_trans; eauto. apply MMap.get_ge; auto.
+  SSSSSSSCase "Didn't overlap offset o, for another reason".
+  simpl in LOAD.
+  erewrite Mem.load_store_other in LOAD; eauto; [|right; left; omega]. merge.
+  destruct (abs b0) as []_eqn; [|contradiction].
+  destruct v; auto.
+  destruct (abs b) as []_eqn.
+  SSSSSSSSCase "abs b = Some".
+  eapply MMap.get_ge; eauto.
+  SSSSSSSSCase "abs b = None".
+  eapply PTSet.ge_trans; eauto. apply MMap.get_ge; auto.
+  SSSSSSCase "Didn't store in b0".
+  simpl in LOAD. erewrite Mem.load_store_other in LOAD; eauto. merge.
+  destruct (abs b0) as []_eqn; [|contradiction].
+  destruct v; auto.
+  destruct (abs b1) as []_eqn.
+  SSSSSSSCase "abs b1 = Some".
+  eapply MMap.get_ge; eauto.
+  SSSSSSSCase "abs b1 = None".
+  eapply PTSet.ge_trans; eauto. apply MMap.get_ge; auto.
+  SSSCase "EF_vload_global".
+  exists abs. constructor; auto.
+  SSSSCase "ok_abs_result".
+  econstructor.
+  SSSSSCase "result".
+  unfold safe_funanalysis. rewrite Heqo. eauto.
+  SSSSSCase "regsat".
+  intros; destruct (peq res r); [subst | eapply regsat_assign_other; eauto;
+    eapply regsat_ge; [eauto | eapply RMap.ge_trans; eauto]].
+  unfold regsat, valsat. rewrite Regmap.gss. destruct v; auto.
+  pose proof load_vptr_Mint32 as LV. specialize (LV chunk m0 (Vptr b ofs) b0 i).
+  feed LV. simpl. auto. subst. destruct (abs b0).
+  admit. admit. admit.
+  (*
+  SSSSSSCase "abs b0 = Some".
+  eapply PTSet.ge_trans. apply RMap.get_ge. eauto.
+  apply RMap.get_add_same. apply PTSet.In_top.
+  SSSSSSCase "abs b0 = None".
+  eapply PTSet.ge_trans. apply RMap.get_ge. eauto. apply RMap.get_add_same.
+  *)
+  SSSSSCase "memsat".
+  eapply memsat_ge; eauto.
+  SSSCase "EF_vstore_global".
+  admit.
+  SSSCase "EF_malloc".
+  exists (fun x =>
+    if zeq x b
+      then Some (Just (Allocs (Just pc)))
+      else abs x).
+  constructor; auto.
+  SSSSCase "ok_stack".
+  erewrite Mem.nextblock_store; [|eauto]. eapply ok_stack_alloc; eauto.
+  SSSSCase "ok_abs_mem".
+  unalias. split; intros.
+  destruct (zeq b0 b); [subst|].
+  eapply Mem.store_valid_block_1; eauto. eapply Mem.valid_new_block; eauto.
+  eapply Mem.store_valid_block_1; eauto. eapply Mem.valid_block_alloc; eauto.
+  apply MEM. auto.
+  destruct (zeq b0 b); [subst|].
+  congruence.
+  apply MEM.
+  eapply Mem.store_valid_block_2 in H2; [|eauto].
+  eapply Mem.valid_block_alloc_inv in H2; [|eauto].
+  inv H2. congruence. auto.
+  SSSSCase "ok_abs_genv".
+  unalias; intros. destruct (zeq b0 b); auto.
+  exfalso. subst. eapply Mem.fresh_block_alloc; eauto. apply MEM.
+  erewrite GENV; [congruence|eauto].
+  SSSSCase "sp".
+  destruct (zeq bsp b); auto.
+  subst. exfalso. eapply Mem.fresh_block_alloc; eauto. apply MEM. congruence.
+  SSSSCase "ok_abs_result".
+  econstructor.
+  SSSSSCase "result".
+  unfold safe_funanalysis. rewrite Heqo. eauto.
+  SSSSSCase "regsat".
+  intros; destruct (peq res r); [subst | ].
+  SSSSSSCase "res = r".
+  unfold regsat, valsat. rewrite Regmap.gss.
+  destruct (zeq b b); [merge|congruence].
+  eapply RMap.get_ge. eauto. apply RMap.get_add_same. apply PTSet.In_singleton.
+  SSSSSSCase "res <> r".
+  unfold regsat, valsat. rewrite Regmap.gso; [|auto]. destruct (rs#r) as []_eqn; auto.
+  regsat_intro rs r. destruct (zeq b0 b).
+  SSSSSSSCase "b0 = b".
+  subst. eapply RMap.get_ge. eauto. destruct (abs b) as []_eqn.
+  SSSSSSSSCase "abs b = Some".
+  exfalso. eapply Mem.fresh_block_alloc; eauto. apply MEM. congruence.
+  SSSSSSSSCase "abs b = None".
+  eapply RMap.get_ge. apply RMap.ge_add. apply IN. apply PTSet.In_top.
+  SSSSSSSCase "b0 <> b".
+  destruct (abs b0) as []_eqn.
+  SSSSSSSSCase "abs b0 = Some".
+  eapply RMap.get_ge. eauto. eapply RMap.get_ge. apply RMap.ge_add. auto.
+  SSSSSSSSCase "abs b0 = None".
+  eapply PTSet.ge_trans. apply RMap.get_ge. eauto.
+  eapply PTSet.ge_trans. apply RMap.get_ge. apply RMap.ge_add. auto.
+  SSSSSCase "memsat".
+  eapply memsat_ge; eauto.
+  unfold memsat, valsat in *. intros.
+  destruct (zeq b0 b).
+  SSSSSSCase "b0 = b".
+  subst. destruct v; auto. simpl in LOAD. pose proof LOAD as LOAD'.
+  eapply Mem.load_pointer_store in LOAD; eauto. intuition; try solve [congruence]; merge.
+  simpl in H0. pose proof (Int.unsigned_range o). omegaContradiction.
+  erewrite Mem.load_store_other in LOAD'; eauto.
+  eapply Mem.load_alloc_same in LOAD'; eauto. inv LOAD'.
+  SSSSSSCase "b0 <> b".
+  simpl in *.
+  erewrite Mem.load_store_other in LOAD; eauto.
+  erewrite Mem.load_alloc_unchanged in LOAD; eauto.
+  specialize (MSAT _ _ _ LOAD). destruct (abs b0) as []_eqn; auto.
+  destruct v; auto. destruct (zeq b1 b); auto.
+  subst. destruct (abs b) as []_eqn.
+  SSSSSSSSCase "abs b = Some".
+  exfalso. eapply Mem.fresh_block_alloc; eauto. apply MEM. congruence.
+  SSSSSSSSCase "abs b = None".
+  apply MSAT. apply PTSet.In_top.
+  SSSSSSCase "b0 <> b".
+  apply MEM. erewrite load_alloc_other' in LOAD; eauto.
+  specialize (MSAT _ _ _ LOAD). destruct (abs b0); auto; congruence.
+  SSSCase "EF_free".
+  exists abs. constructor; auto.
+  SSSSCase "ok_stack".
+  erewrite Mem.nextblock_free; eauto.
+  SSSSCase "ok_abs_mem".
+  eapply ok_abs_mem_free; eauto.
+  SSSSCase "ok_abs_result".
+  econstructor.
+  SSSSSCase "result".
+  unfold safe_funanalysis. rewrite Heqo. eauto.
+  SSSSSCase "regsat".
+  intros; destruct (peq res r); [subst | eapply regsat_assign_other; eauto;
+    eapply regsat_ge; [eauto | eapply RMap.ge_trans; eauto]].
+  unfold regsat, valsat. rewrite Regmap.gss. auto.
+  SSSSSCase "memsat".
+  eapply memsat_ge; eauto. eapply memsat_free; eauto.
+  SSSCase "EF_memcpy".
+  exists abs. constructor; auto.
+  SSSSCase "ok_stack".
+  erewrite Mem.nextblock_storebytes; eauto.
+  SSSSCase "ok_abs_mem".
+  eapply ok_abs_mem_storebytes; eauto.
+  SSSSCase "ok_abs_result".
+  econstructor.
+  SSSSSCase "result".
+  unfold safe_funanalysis. rewrite Heqo. eauto.
+  SSSSSCase "regsat".
+  intros; destruct (peq res r); [subst | eapply regsat_assign_other; eauto;
+    eapply regsat_ge; [eauto | eapply RMap.ge_trans; eauto]].
+  unfold regsat, valsat. rewrite Regmap.gss. auto.
+  SSSSSCase "memsat".
+  eapply memsat_ge; eauto.
+  unfold memsat, valsat in *. intros.
+  repeat (destruct args; try solve [inv H]). inv H. inv H0.
+  destruct (zeq b bdst).
+  SSSSSSCase "b = bdst".
+  subst. regsat_intro rs r. destruct (abs bdst) as []_eqn.
+  SSSSSSSCase "abs bdst = Some".
+  destruct v; auto. destruct (abs b) as []_eqn.
+  SSSSSSSSCase "abs b = Some".
+  apply In_add_ptset_to_image. apply PTSet.In_top. eapply In_unknown_offset; eauto.
+  SSSSSSSSCase "abs b = None".
+  eapply PTSet.ge_trans. repeat intro. apply In_add_ptset_to_image. apply H.
+  eapply In_unknown_offset; eauto. apply PTSet.ge_refl. apply PTSet.eq_refl.
+  SSSSSSSCase "abs bdst = None".
+  eapply Mem.load_valid_access in LOAD. eapply Mem.valid_access_implies in LOAD.
+  eapply Mem.valid_access_valid_block in LOAD.
+  eapply Mem.storebytes_valid_block_2 in LOAD; eauto.
+  apply MEM in LOAD. congruence. constructor.
+  SSSSSSCase "b <> bdst".
+  specialize (MSAT b o v). feed MSAT. simpl. erewrite <- Mem.load_storebytes_other; eauto.
+  destruct (abs b); [|contradiction]. destruct v; auto. destruct (abs b0).
+  SSSSSSSCase "abs b0 = Some".
+  eapply MMap.get_ge. apply ge_add_ptset_to_image. auto.
+  SSSSSSSCase "abs b0 = None".
+  eapply PTSet.ge_trans. eapply MMap.get_ge. eapply ge_add_ptset_to_image. auto.
+  SSSCase "EF_annot".
+  exists abs. constructor; auto.
+  SSSSCase "ok_abs_result".
+  econstructor.
+  SSSSSCase "result".
+  unfold safe_funanalysis. rewrite Heqo. eauto.
+  SSSSSCase "regsat".
+  intros; destruct (peq res r); [subst | eapply regsat_assign_other; eauto;
+    eapply regsat_ge; [eauto | eapply RMap.ge_trans; eauto]].
+  unfold regsat, valsat. rewrite Regmap.gss. auto.
+  SSSSSCase "memsat".
+  eapply memsat_ge; eauto.
+  SSSCase "EF_annot_val".
+  exists abs. constructor; auto.
+  SSSSCase "ok_abs_result".
+  econstructor.
+  SSSSSCase "result".
+  unfold safe_funanalysis. rewrite Heqo. eauto.
+  SSSSSCase "regsat".
+  intros; destruct (peq res r); [subst | eapply regsat_assign_other; eauto;
+    eapply regsat_ge; [eauto | eapply RMap.ge_trans; eauto]].
+  unfold regsat, valsat. rewrite Regmap.gss. destruct v; auto.
+  inv H1. specialize (GENV _ _ H5). rewrite GENV.
+  destruct args. inv H. destruct args; inv H. inv H0.
+  regsat_intro rs r0. rewrite GENV in IN.
+  eapply RMap.get_ge. eauto. apply RMap.get_add_same. auto.
+  SSSSSCase "memsat".
+  eapply memsat_ge; eauto. eapply MMap.ge_trans; eauto.
+  SCase "Kildall failed".
+  rewrite PMap.gi in RPC. inv RPC.
+  inv STEP; try solve [
+    exists abs; constructor; auto; econstructor; eauto;
+      unfold safe_funanalysis; rewrite Heqo; rewrite PMap.gi; reflexivity
+  ].
+  SSCase "Iop".
+  exists abs; constructor; auto.
+  SSSCase "ok_abs_result".
+  econstructor.
+  SSSSCase "result".
+  unfold safe_funanalysis. rewrite Heqo. rewrite PMap.gi. reflexivity.
+  SSSSCase "regsat".
+  apply regsat_top.
+  SSSSCase "memsat".
+  apply memsat_top. auto.
+  SSCase "Iload".
+  exists abs; constructor; auto.
+  SSSCase "ok_abs_result".
+  econstructor.
+  SSSSCase "result".
+  unfold safe_funanalysis. rewrite Heqo. rewrite PMap.gi. reflexivity.
+  SSSSCase "regsat".
+  apply regsat_top.
+  SSSSCase "memsat".
+  apply memsat_top. auto.
+  SSCase "Istore".
+  destruct a; try solve [inv H14].
+  exists abs; constructor; auto.
+  SSSCase "ok_stack".
+  erewrite Mem.nextblock_store; eauto.
+  SSSCase "ok_abs_mem".
+  eapply ok_abs_mem_store; eauto.
+  SSSCase "ok_abs_result".
+  econstructor.
+  SSSSCase "result".
+  unfold safe_funanalysis. rewrite Heqo. rewrite PMap.gi. reflexivity.
+  SSSSCase "regsat".
+  apply regsat_top.
+  SSSSCase "memsat".
+  apply memsat_top. eapply ok_abs_mem_store; eauto.
+  SSCase "Ibuiltin".
+  destruct ef; inv H13; merge; try solve [
+    exists abs; constructor; auto; econstructor;
+    [ unfold safe_funanalysis; rewrite Heqo; rewrite PMap.gi; reflexivity
+    | apply regsat_top
+    | apply memsat_top; auto
+    ]
+  ].
+  inv H0.
+  SSSCase "EF_vstore (volatile)".
+  admit.
+  SSSCase "EF_vstore (not volatile)".
+  exists abs. constructor; auto.
+  SSSSCase "ok_stack".
+  erewrite Mem.nextblock_store; eauto.
+  SSSSCase "ok_abs_mem".
+  eapply ok_abs_mem_store; eauto.
+  SSSSCase "ok_abs_result".
+  econstructor.
+  SSSSSCase "result".
+  unfold safe_funanalysis. rewrite Heqo. rewrite PMap.gi. reflexivity.
+  SSSSSCase "regsat".
+  apply regsat_top.
+  SSSSSCase "memsat".
+  apply memsat_top. eapply ok_abs_mem_store; eauto.
+  SSSCase "EF_vstore_global".
+  admit.
+  SSSCase "EF_malloc".
+  exists (fun x =>
+    if zeq x b
+      then Some (Just (Allocs (Just pc)))
+      else abs x).
+  (* We will need this twice, so let's prove it upfront... *)
+  assert (OKAM:
+    ok_abs_mem
+    (fun x : Z => if zeq x b then Some (Some (Allocs (Some pc))) else abs x)
+    m0).
+  unalias. split; intros.
+  destruct (zeq b0 b); [subst|].
+  eapply Mem.store_valid_block_1; eauto. eapply Mem.valid_new_block; eauto.
+  eapply Mem.store_valid_block_1; eauto. eapply Mem.valid_block_alloc; eauto.
+  apply MEM. auto.
+  destruct (zeq b0 b); [subst|].
+  congruence.
+  apply MEM.
+  eapply Mem.store_valid_block_2 in H2; [|eauto].
+  eapply Mem.valid_block_alloc_inv in H2; [|eauto].
+  inv H2. congruence. auto.
+  constructor; auto.
+  SSSSCase "ok_stack".
+  erewrite Mem.nextblock_store; [|eauto]. eapply ok_stack_alloc; eauto.
+  SSSSCase "ok_abs_genv".
+  unalias; intros. destruct (zeq b0 b); auto.
+  exfalso. subst. eapply Mem.fresh_block_alloc; eauto. apply MEM.
+  erewrite GENV; [congruence|eauto].
+  SSSSCase "sp".
+  destruct (zeq bsp b); auto.
+  subst. exfalso. eapply Mem.fresh_block_alloc; eauto. apply MEM. congruence.
+  SSSSCase "ok_abs_result".
+  econstructor.
+  SSSSSCase "result".
+  unfold safe_funanalysis. rewrite Heqo. rewrite PMap.gi. reflexivity.
+  SSSSSCase "regsat".
+  apply regsat_top.
+  SSSSSCase "memsat".
+  apply memsat_top. auto.
+  SSSCase "EF_free".
+  exists abs. constructor; auto.
+  SSSSCase "ok_stack".
+  erewrite Mem.nextblock_free; eauto.
+  SSSSCase "ok_abs_mem".
+  eapply ok_abs_mem_free; eauto.
+  SSSSCase "ok_abs_result".
+  econstructor.
+  SSSSSCase "result".
+  unfold safe_funanalysis. rewrite Heqo. rewrite PMap.gi. reflexivity.
+  SSSSSCase "regsat".
+  apply regsat_top.
+  SSSSSCase "memsat".
+  apply memsat_top. eapply ok_abs_mem_free; eauto.
+  SSSCase "EF_memcpy".
+  exists abs. constructor; auto.
+  SSSSCase "ok_stack".
+  erewrite Mem.nextblock_storebytes; eauto.
+  SSSSCase "ok_abs_mem".
+  eapply ok_abs_mem_storebytes; eauto.
+  SSSSCase "ok_abs_result".
+  econstructor.
+  SSSSSCase "result".
+  unfold safe_funanalysis. rewrite Heqo. rewrite PMap.gi. reflexivity.
+  SSSSSCase "regsat".
+  apply regsat_top.
+  SSSSSCase "memsat".
+  apply memsat_top.
+  eapply ok_abs_mem_storebytes; eauto.
+
+  Case "state -> callstate".
+  exists abs. inv STEP.
+  SCase "Icall".
+  constructor; auto.
+  SSCase "ok_stack".
+  econstructor; eauto.
+  SSSCase "MEM".
+  apply MEM.
+  SSSCase "ok_abs_result_stack".
+  unfold safe_funanalysis in RPC. destruct (funanalysis f) as []_eqn.
+  SSSSCase "Kildall terminated".
+  pose proof Heqo as FPS.
+  eapply Solver.fixpoint_solution with (n:=pc)(s:=pc') in FPS; [|
+    unfold successors; unfold successors_list; rewrite PTree.gmap1;
+      rewrite H6; simpl; auto; eapply list_nth_z_in; eauto].
+  unfold transf in FPS. rewrite H6 in FPS. unfold Solver.L.ge in FPS.
+  destruct (t#pc') as [rmap' mmap']_eqn. rewrite RPC in FPS. destruct FPS as [RGE MGE].
+  econstructor.
+  SSSSSCase "result".
+  unfold safe_funanalysis. rewrite Heqo. eauto.
+  SSSSSCase "regsat".
+  eapply regsat_ge; eauto. eapply RMap.ge_trans; eauto. apply RMap.ge_add.
+  SSSSSCase "ret".
+  eapply PTSet.ge_trans. apply RMap.get_ge; eauto.
+  eapply PTSet.ge_trans. apply RMap.get_add_same. auto with ptset.
+  SSSSSCase "mem".
+  auto. (*?*)
+  SSSSCase "Kildall failed".
+  econstructor.
+  SSSSSCase "result".
+  unfold safe_funanalysis. rewrite Heqo. rewrite PMap.gi. unfold Result.top. eauto.
+  SSSSSCase "regsat".
+  eapply regsat_ge; eauto. apply RMap.ge_top.
+  SSSSSCase "ret".
+  apply RMap.get_top.
+  SSSSSCase "mem".
+  apply MMap.eq_refl.
+  SCase "Itailcall".
+  constructor; auto.
+  SSCase "ok_abs_mem".
+  eapply ok_abs_mem_free; eauto.
+  SSCase "ok_stack".
+  erewrite Mem.nextblock_free; eauto.
+
+  Case "state -> returnstate".
+  exists abs. inv STEP.
+  constructor; auto.
+  SCase "ok_abs_mem".
+  eapply ok_abs_mem_free; eauto.
+  SCase "ok_stack".
+  erewrite Mem.nextblock_free; eauto.
+
+  Case "callstate -> state".
+  inv STEP.
+  exists (fun b =>
+    if zeq b stk then Some (Just Stack) else
+      match abs b with
+      | Some ab => Some (Just
+        (
+          match ab with
+          | Just (Globals (Some i)) => Globals (Some i)
+          | Just (Globals None)     => Globals None
+          | _                       => Other
+          end
+        ))
+      | None    => None
+      end
+  ).
+  constructor; auto.
+  SCase "ok_stack".
+  eapply ok_stack_alloc; eauto.
+  SCase "ok_abs_mem".
+  unalias; split; intros.
+  SSCase "->".
+  destruct (zeq b stk).
+  SSSCase "b = stk".
+  subst. eapply Mem.valid_new_block; eauto.
+  SSSCase "b <> stk".
+  destruct (abs b) as []_eqn; [|congruence].
+  eapply Mem.valid_block_alloc; eauto. apply MEM. congruence.
+  SSCase "<-".
+  destruct (zeq b stk).
+  SSSCase "b = stk".
+  congruence.
+  SSSCase "b <> stk".
+  destruct (abs b) as []_eqn. destruct a; congruence.
+  eapply Mem.valid_block_alloc_inv in H; eauto. intuition. apply MEM in H1; auto.
+  SCase "ok_abs_genv".
+  unalias; intros. specialize (GENV _ _ FIND). rewrite GENV.
+  destruct (zeq b stk); [|auto]. subst.
+  exfalso. eapply Mem.fresh_block_alloc; eauto. apply MEM. congruence.
+  SCase "sp".
+  destruct (zeq stk stk); [auto|congruence].
+  SCase "ok_abs_result".
+  destruct (funanalysis f0) as []_eqn.
+  SSCase "Kildall will terminate".
+  destruct t. destruct t. pose proof Heqo as FA.
+  eapply Solver.fixpoint_entry in Heqo; [|constructor; eauto].
+  destruct ((t, t1, t0) # (fn_entrypoint f0)) as [rmap mmap]_eqn.
+  setoid_rewrite Heqp in Heqo. unfold entry_result in Heqo.
+  destruct Heqo as [RGE MGE].
+  econstructor.
+  SSSCase "result".
+  unfold safe_funanalysis. rewrite FA. eauto.
+  SSSCase "regsat".
+  eapply regsat_ge; eauto.
+  generalize (fn_params f0). intros. unalias.
+  destruct ((init_regs args l)#r) as []_eqn; auto.
+  assert (InA eq r l).
+  SSSSCase "assert".
+  revert Heqv. revert args. induction l; intros.
+  simpl in Heqv. rewrite Regmap.gi in Heqv. congruence.
+  simpl in Heqv. destruct args.
+  rewrite Regmap.gi in Heqv. congruence.
+  destruct (peq r a).
+  subst. constructor. auto.
+  rewrite Regmap.gso in Heqv; [|auto]. right. eapply IHl; eauto.
+  SSSSCase "end of assert".
+  unfold entry_rmap. destruct (zeq b stk).
+  subst.
+  eapply fold_left_adds_prop; eauto; intros.
+  apply RMap.get_add_same. apply PTSet.In_top.
+  apply RMap.get_add. auto.
+  destruct (abs b).
+  eapply fold_left_adds_prop; eauto; intros.
+  apply RMap.get_add_same. apply PTSet.In_top.
+  apply RMap.get_add. auto.
+  eapply fold_left_adds_prop; eauto; intros.
+  apply RMap.get_add_same.
+  eapply PTSet.ge_trans. apply RMap.get_add. auto.
+  SSSCase "memsat".
+  eapply memsat_ge; eauto. unalias. intros. destruct (zeq b stk).
+  SSSSCase "b = stk".
+  subst. simpl in LOAD. eapply Mem.load_alloc_same in LOAD; eauto. subst. auto.
+  SSSSCase "b <> stk".
+  destruct (abs b) as []_eqn.
+  SSSSSCase "abs b = Some".
+  destruct v; auto.
+  destruct (zeq b0 stk).
+  SSSSSSCase "b0 = stk".
+  subst. unfold entry_mmap.
+  destruct a; try destruct a; try destruct o0; first
+    [ solve [apply MMap.get_add_overlap; [compute; auto | apply PTSet.In_top]]
+    | solve [apply MMap.get_add; apply MMap.get_add_overlap;
+      [compute; auto | apply PTSet.In_top]]
+    ].
+  SSSSSSCase "b0 <> stk".
+  destruct (abs b0) as []_eqn.
+  SSSSSSSCase "abs b0 = Some".
+  unfold entry_mmap.
+  destruct a; try destruct a; try destruct o0; first
+    [ solve [apply MMap.get_add_overlap; [compute; auto | apply PTSet.In_top]]
+    | solve [apply MMap.get_add; apply MMap.get_add_overlap;
+      [compute; auto | apply PTSet.In_top]]
+    ].
+  SSSSSSSCase "abs b0 = None".
+  unfold entry_mmap.
+  destruct a; try destruct a; try destruct o0; first
+    [ solve [apply MMap.get_add_overlap; compute; auto]
+    | solve [eapply PTSet.ge_trans;
+      [apply MMap.get_add | apply MMap.get_add_overlap; compute; auto]]
+    ].
+  SSSSSCase "abs b = None".
+  eapply load_valid_block in LOAD. eapply Mem.valid_block_alloc_inv in LOAD; eauto.
+  intuition. apply MEM in H; auto.
+  SSCase "Kildall won't terminate".
+  econstructor; intros.
+  SSSCase "result".
+  unfold safe_funanalysis. rewrite Heqo. rewrite PMap.gi. unfold Result.top. auto.
+  SSSCase "regsat".
+  unalias.
+  destruct ((init_regs args (fn_params f0))#r); auto.
+  destruct (zeq b stk).
+  subst. apply RMap.get_top. apply PTSet.In_top.
+  destruct (abs b); apply RMap.get_top; apply PTSet.In_top.
+  SSSCase "memsat".
+  unalias. intros. destruct (zeq b stk).
+  SSSSCase "b = stk".
+  subst. destruct v; auto. simpl in LOAD. eapply Mem.load_alloc_same in LOAD; eauto.
+  congruence.
+  SSSSCase "b <> stk".
+  destruct (abs b) as []_eqn.
+  SSSSSCase "abs b = Some".
+  destruct v; auto.
+  destruct (zeq b0 stk).
+  SSSSSSCase "b0 = stk".
+  subst. apply MMap.get_top. apply PTSet.In_top.
+  SSSSSSCase "b0 <> stk".
+  destruct (abs b0) as []_eqn.
+  apply MMap.get_top. apply PTSet.In_top.
+  apply MMap.get_eq_top. apply MMap.eq_refl.
+  SSSSSCase "abs b = None".
+  eapply load_valid_block in LOAD. eapply Mem.valid_block_alloc_inv in LOAD; eauto.
+  intuition. apply MEM in H; auto.
+
+  Case "callstate -> returnstate (un-inlined external calls)".
+  inv STEP. destruct ef; inv H4; try solve [exists abs; constructor; auto].
+  SCase "volatile store".
+  exists abs; constructor; auto.
+  admit. (* eapply ok_abs_mem_store; eauto. *)
+  admit. (* erewrite Mem.nextblock_store; eauto. *)
+  SCase "global volatile store".
+  exists abs; constructor; auto.
+  admit. (* eapply ok_abs_mem_store; eauto. *)
+  admit. (* erewrite Mem.nextblock_store; eauto. *)
+  SCase "malloc".
+  exists (fun x =>
+    if zeq x b
+      then Some (Just Other)
+      else abs x).
+  constructor; auto.
+  SSCase "ok_abs_mem".
+  constructor; intros.
+  destruct (zeq b0 b).
+  subst. eapply Mem.store_valid_block_1; eauto. eapply Mem.valid_new_block; eauto.
+  eapply Mem.store_valid_block_1; eauto. eapply Mem.valid_block_alloc; eauto. apply MEM.
+  auto.
+  destruct (zeq b0 b).
+  congruence.
+  apply MEM. eapply Mem.store_valid_block_2 in H1; [|eauto].
+  eapply Mem.valid_block_alloc_inv in H1; eauto.
+  intuition.
+  SSCase "ok_stack".
+  erewrite Mem.nextblock_store; [|eauto]. eapply ok_stack_alloc; eauto.
+  SSCase "ok_abs_genv".
+  unalias; intros. specialize (GENV _ _ FIND). destruct (zeq b0 b); [|auto].
+  subst. exfalso. eapply Mem.fresh_block_alloc; eauto. apply MEM. congruence.
+  SCase "free".
+  exists abs; constructor; auto.
+  SSCase "ok_abs_mem".
+  eapply ok_abs_mem_free; eauto.
+  SSCase "ok_stack".
+  erewrite Mem.nextblock_free; eauto.
+  SCase "memcpy".
+  exists abs; constructor; auto.
+  SSCase "ok_abs_mem".
+  constructor; intros.
+  eapply Mem.storebytes_valid_block_1; eauto. apply MEM. auto.
+  apply MEM. eapply Mem.storebytes_valid_block_2; eauto.
+  erewrite Mem.nextblock_storebytes; eauto.
+
+  Case "returnstate -> state".
+  inv STEP.
+  clear MEM GENV abs. (* don't even think about using this abs! *)
+  inv STK. (* use this good old abs instead! *)
+  exists (fun b =>
+    match abs b with
+    | Some _ => abs b
+    | None   => if (zlt b (Mem.nextblock m0)) then Some (Just Other) else None
+    end).
+  econstructor; eauto; intros.
+  SCase "ok_abs_mem".
+  constructor; intros.
+  specialize (MEM b). destruct (abs b). red. apply MEM. auto.
+  destruct (zlt b (Mem.nextblock m0)). auto. congruence.
+  destruct (abs b) as []_eqn. congruence.
+  destruct (zlt b (Mem.nextblock m0)); congruence.
+  SCase "ok_abs_genv".
+  unalias; intros. specialize (GENV _ _ FIND). rewrite GENV. auto.
+  SCase "sp".
+  rewrite SP. auto.
+  SCase "ok_abs_result".
+  inv RES.
+  econstructor; eauto; intros.
+  SSCase "regsat".
+  unalias. destruct (peq res r); [subst|].
+  SSSCase "res = r".
+  rewrite Regmap.gss. destruct v; auto.
+  destruct (abs b). apply RET. auto with ptset.
+  destruct (zlt b (Mem.nextblock m0)); [|auto].
+  apply RET. auto with ptset.
+  SSSCase "res <> r".
+  specialize (RSAT r). rewrite Regmap.gso; [|auto]. destruct (rs0#r); auto.
+  destruct (abs b). auto.
+  destruct (zlt b (Mem.nextblock m0)); [|auto].
+  apply RSAT. auto with ptset.
+  SSCase "memsat".
+  unalias. intros. destruct (abs b). destruct v0; auto.
+  destruct (abs b0); destruct (zlt b0 (Mem.nextblock m0));
+  apply MMap.get_eq_top; auto with ptset.
+  destruct (zlt b (Mem.nextblock m0)). destruct v0; auto.
+  destruct (abs b0).
+  apply MMap.get_eq_top; auto with ptset.
+  destruct (zlt b0 (Mem.nextblock m0));
+  apply MMap.get_eq_top; auto with ptset.
+  apply load_valid_block in LOAD. congruence.
+Qed.
